doc/coq/Concrete.v
@@ -4,8 +4,6 @@ Definition time := nat.
 
 Definition path := list time.
 
-Definition update_t (t : time) := S t.
-
 Definition eq_t (t1 t2 : time) := t1 =? t2.
 
 Fixpoint eq_p (p1 p2 : path) :=
@@ -18,22 +16,12 @@ Fixpoint eq_p (p1 p2 : path) :=
                     else false
   end.
 
-Definition len_p (p : path) := List.length p.
-
 Inductive dy_ctx :=
   | dy_c_hole
   | dy_c_lam (x: expr_id) (tx : time) (C : dy_ctx)
   | dy_c_lete (x : expr_id) (tx : time) (C : dy_ctx)
   | dy_c_letm (M : mod_id) (CM : dy_ctx) (C : dy_ctx)
 .
-
-Fixpoint dy_plugin_c Cout Cin :=
-  match Cout with
-  | dy_c_hole => Cin
-  | dy_c_lam x tx C' => dy_c_lam x tx (dy_plugin_c C' Cin)
-  | dy_c_lete x tx C' => dy_c_lete x tx (dy_plugin_c C' Cin)
-  | dy_c_letm M CM C' => dy_c_letm M CM (dy_plugin_c C' Cin)
-  end.
 
 Fixpoint dy_level (C : dy_ctx) : path :=
   match C with
@@ -43,17 +31,12 @@ Fixpoint dy_level (C : dy_ctx) : path :=
   | dy_c_letm _ _  C' => dy_level C'
   end.
 
-Fixpoint ctx_x (C : dy_ctx) (x : expr_id) :=
-  match C with
-  | dy_c_hole => dy_c_hole
-  | dy_c_lam x' tx' C'
-  | dy_c_lete x' tx' C' =>
-    match ctx_x C' x with
-    | dy_c_hole => if eq_eid x x' then dy_c_lam x tx' dy_c_hole
-                   else dy_c_hole
-    | C'' => dy_c_lam x' tx' C''
-    end
-  | dy_c_letm M CM C' => ctx_x C' x
+Fixpoint dy_plugin_c Cout Cin :=
+  match Cout with
+  | dy_c_hole => Cin
+  | dy_c_lam x tx C' => dy_c_lam x tx (dy_plugin_c C' Cin)
+  | dy_c_lete x tx C' => dy_c_lete x tx (dy_plugin_c C' Cin)
+  | dy_c_letm M CM C' => dy_c_letm M CM (dy_plugin_c C' Cin)
   end.
 
 Fixpoint addr_x (C : dy_ctx) (x : expr_id) :=
@@ -68,35 +51,6 @@ Fixpoint addr_x (C : dy_ctx) (x : expr_id) :=
   | dy_c_letm _ _ C' => addr_x C' x
   end.
 
-Lemma addr_is_level :
-  forall x C, addr_x C x = dy_level (ctx_x C x).
-Proof.
-  assert (forall C x, match ctx_x C x with dy_c_letm _ _ _ => False | _ => True end) as contra.
-  { induction C; intros x'; simpl; eauto
-    ; try destruct (ctx_x C x'); simpl; try destruct (eq_eid x' x); simpl; eauto.
-    apply IHC2. }
-  intros x. induction C; simpl; try rewrite IHC; eauto;
-  remember (ctx_x C x) as ctxX; destruct ctxX; simpl; eauto;
-  remember (eq_eid x x0) as eq; destruct eq; simpl; eauto;
-  try (remember (dy_level ctxX ++ [tx0]) as l; destruct l; simpl; eauto).
-  - assert (In tx0 (dy_level ctxX ++ [tx0])). 
-    apply in_app_iff; right; simpl; eauto.
-    rewrite <- Heql in H. inversion H.
-  - assert (In tx0 (dy_level ctxX ++ [tx0])). 
-    apply in_app_iff; right; simpl; eauto.
-    rewrite <- Heql in H. inversion H.
-  - specialize (contra C x). rewrite <- HeqctxX in contra. inversion contra.
-  - specialize (contra C x). rewrite <- HeqctxX in contra. inversion contra.
-  - assert (In tx0 (dy_level ctxX ++ [tx0])). 
-    apply in_app_iff; right; simpl; eauto.
-    rewrite <- Heql in H. inversion H.
-  - assert (In tx0 (dy_level ctxX ++ [tx0])). 
-    apply in_app_iff; right; simpl; eauto.
-    rewrite <- Heql in H. inversion H.
-  - specialize (contra C x). rewrite <- HeqctxX in contra. inversion contra.
-  - specialize (contra C x). rewrite <- HeqctxX in contra. inversion contra.
-Qed.
-
 Fixpoint ctx_M (C : dy_ctx) (M : mod_id) :=
   match C with
   | dy_c_hole => None
@@ -109,9 +63,14 @@ Fixpoint ctx_M (C : dy_ctx) (M : mod_id) :=
     end
   end.
 
-(* a term, a proof, a path, a context *)
+(* a term, a context *)
 Inductive expr_value :=
-  | Val (v : expr_tm) (pf : value v) (C : dy_ctx)
+  | Closure (x : expr_id) (e : tm) (C : dy_ctx)
+.
+
+Inductive dy_value :=
+  | EVal (ev : expr_value)
+  | MVal (mv : dy_ctx)
 .
 
 Inductive state :=
@@ -119,8 +78,14 @@ Inductive state :=
        (t : time)
 .
 
+Definition update_t (C : dy_ctx) (st : state) 
+                    (x : expr_id) (v : expr_value) :=
+  match st with
+  | ST mem t => S t
+  end.
+
 Definition update_m {X} mem (p : path) (x : X) :=
-  fun p1 => if eq_p p1 p then Some x else mem p1.
+  fun p' => if eq_p p' p then Some x else mem p'.
 
 Definition empty_mem {X} (p : path) : option X := None.
 
@@ -131,550 +96,474 @@ Notation "Cout '[|' Cin '|]'" := (dy_plugin_c Cout Cin)
                               (at level 100, Cin at next level, right associativity).
 Notation "'[||]'" := (dy_c_hole) (at level 100).
 
-Inductive EevalR (C : dy_ctx) (st : state)
-    : expr_tm -> expr_value -> state -> Prop :=
-  | Eeval_var x v mem t
+Inductive EvalR (C : dy_ctx) (st : state)
+    : tm -> dy_value -> state -> Prop :=
+  | Eval_var_e x v mem t
              (STATE : ST mem t = st)
              (ADDR : [] <> addr_x C x)
              (ACCESS : Some v = mem (addr_x C x))
-    : EevalR C st (e_var x) v st
-  | Eeval_lam x e
-    : EevalR C st (e_lam x e)
-            (Val (e_lam x e) (v_fn x e) C) st
-  | Eeval_app e1 e2 
-              x e C_lam st_lam
-              arg mem t
-              v st_v
-              (FN : EevalR C st e1
-                           (Val (e_lam x e) (v_fn x e) C_lam) st_lam)
-              (ARG : EevalR C st_lam e2
-                            arg (ST mem t))
-              (BODY : EevalR (C_lam [|dy_c_lam x t  ([||])|])
-                             (ST (t :: (dy_level C_lam) !-> arg ; mem) (update_t t))
-                              e v st_v)
-    : EevalR C st (e_app e1 e2) v st_v
-  | Eeval_link m e C_m st_m v st_v
-               (MOD : MevalR C st m C_m st_m)
-               (LINK : EevalR C_m st_m e v st_v)
-    : EevalR C st (e_link m e) v st_v
-
-with MevalR (C : dy_ctx) (st : state)
-    : mod_tm -> dy_ctx -> state -> Prop :=
-  | Meval_empty
-    : MevalR C st m_empty C st
-  | Meval_var M C_M (ACCESS : Some C_M = ctx_M C M)
-    : MevalR C st (m_var M) C_M st
-  | Meval_lete x e v_e mem t
-               m C_m st_m
-               (EVALe : EevalR C st e v_e (ST mem t))
-               (EVALm : MevalR (C [|dy_c_lete x t ([||])|]) 
-                        (ST (t :: (dy_level C) !-> v_e ; mem) (update_t t))
-                        m C_m st_m)
-    : MevalR C st (m_lete x e m) C_m st_m
-  | Meval_letm M m1 C_m1 st_m1
-               m2 C_m2 st_m2
-               (EVALm1 : MevalR C st m1 C_m1 st_m1)
-               (EVALm2 : MevalR (C [|dy_c_letm M C_m1 ([||])|]) st_m1
-                         m2 C_m2 st_m2)
-    : MevalR C st (m_letm M m1 m2) C_m2 st_m2
+    : EvalR C st (e_var x) (EVal v) st
+  | Eval_lam x e
+    : EvalR C st (e_lam x e)
+            (EVal (Closure x e C)) st
+  | Eval_app e1 e2 
+             x e C_lam st_lam
+             arg mem t
+             v st_v
+             (FN : EvalR C st e1
+                         (EVal (Closure x e C_lam)) st_lam)
+             (ARG : EvalR C st_lam e2
+                          (EVal arg) (ST mem t))
+             (BODY : EvalR (C_lam [|dy_c_lam x t ([||])|])
+                           (ST (t :: (dy_level C_lam) !-> arg ; mem) 
+                               (update_t C (ST mem t) x arg))
+                           e (EVal v) st_v)
+    : EvalR C st (e_app e1 e2) (EVal v) st_v
+  | Eval_link m e C_m st_m v st_v
+               (MOD : EvalR C st m (MVal C_m) st_m)
+               (LINK : EvalR C_m st_m e (EVal v) st_v)
+    : EvalR C st (e_link m e) (EVal v) st_v
+  | Eval_empty
+    : EvalR C st m_empty (MVal C) st
+  | Eval_var_m M C_M (ACCESS : Some C_M = ctx_M C M)
+    : EvalR C st (m_var M) (MVal C_M) st
+  | Eval_lete x e v mem t
+              m C_m st_m
+               (EVALe : EvalR C st e (EVal v) (ST mem t))
+               (EVALm : EvalR (C [|dy_c_lete x t ([||])|])
+                        (ST (t :: (dy_level C) !-> v ; mem) 
+                            (update_t C (ST mem t) x v))
+                        m (MVal C_m) st_m)
+    : EvalR C st (m_lete x e m) (MVal C_m) st_m
+  | Eval_letm M m' C' st'
+              m'' C'' st''
+              (EVALm' : EvalR C st m' (MVal C') st')
+              (EVALm'' : EvalR (C [|dy_c_letm M C' ([||])|]) st'
+                         m'' (MVal C'') st'')
+    : EvalR C st (m_letm M m' m'') (MVal C'') st''
 .
 
-Scheme EevalR_ind_mut := Induction for EevalR Sort Prop
-with MevalR_ind_mut := Induction for MevalR Sort Prop.
+Inductive interpreter_state :=
+  | Pending (C : dy_ctx) (st : state) (e : tm)
+  | Error (C : dy_ctx) (st : state) (e : tm) (* Type error *)
+  | Resolved (v : dy_value) (st : state)
+.
+
+Fixpoint eval (C : dy_ctx) (st : state) 
+              (e : tm) (FUEL : nat) :=
+  match FUEL with
+  | 0 => Pending C st e
+  | S FUEL' =>
+    match e with
+    | e_var x =>
+      match addr_x C x with
+      | [] => Error C st e
+      | p => 
+        match st with
+        | ST mem _ =>
+          match mem p with
+          | None => Pending C st e
+          | Some v => Resolved (EVal v) st
+          end
+        end
+      end
+    | e_lam x e' =>
+      Resolved (EVal (Closure x e' C)) st
+    | e_app e1 e2 =>
+      match eval C st e1 FUEL' with
+      | Resolved (EVal (Closure x e' C_lam)) st_lam =>
+        match eval C st_lam e2 FUEL' with
+        | Resolved (EVal arg) (ST mem t) =>
+          match eval (C_lam [| dy_c_lam x t ([||]) |]) 
+                     (ST (t :: (dy_level C_lam) !-> arg ; mem) 
+                         (update_t C (ST mem t) x arg)) 
+                     e' FUEL' with
+          | Resolved (EVal v) st' => Resolved (EVal v) st'
+          | Resolved _ _ => Error C st e
+          | other => other
+          end
+        | Resolved _ _ => Error C st e
+        | other => other
+        end
+      | Resolved _ _ => Error C st e
+      | other => other
+      end
+    | e_link m e' =>
+      match eval C st m FUEL' with
+      | Resolved (MVal C_m) st_m =>
+        match eval C_m st_m e' FUEL' with
+        | Resolved (EVal v) st' => Resolved (EVal v) st'
+        | Resolved _ _ => Error C st e
+        | other => other
+        end
+      | Resolved _ _ => Error C st e
+      | other => other
+      end
+    | m_empty => Resolved (MVal C) st
+    | m_var M =>
+      match ctx_M C M with
+      | None => Pending C st e
+      | Some C_M => Resolved (MVal C_M) st
+      end
+    | m_lete x e m =>
+      match eval C st e FUEL' with
+      | Resolved (EVal v) (ST mem t) =>
+        match eval (C[| dy_c_lete x t ([||]) |]) 
+                   (ST (t :: (dy_level C) !-> v ; mem) 
+                       (update_t C (ST mem t) x v)) 
+                   m FUEL' with
+        | Resolved (MVal C') st' => Resolved (MVal C') st'
+        | Resolved _ _ => Error C st e 
+        | other => other
+        end
+      | Resolved _ _ => Error C st e
+      | other => other
+      end
+    | m_letm M m1 m2 =>
+      match eval C st m1 FUEL' with
+      | Resolved (MVal C') st' =>
+        match eval (C[| dy_c_letm M C' ([||]) |])
+                   st' m2 FUEL' with
+        | Resolved (MVal C'') st'' => Resolved (MVal C'') st''
+        | Resolved _ _ => Error C st e
+        | other => other
+        end
+      | Resolved _ _ => Error C st e
+      | other => other
+      end
+    end
+  end.
+
+Compute eval ([||]) (ST empty_mem 0) 
+             (e_app (e_lam (eid 0) 
+                        (e_app (e_var (eid 0))
+                                (e_var (eid 0))))
+                    (e_lam (eid 0) 
+                        (e_app (e_var (eid 0))
+                                (e_var (eid 0))))) 5. 
+
+Lemma relax_fuel :
+  forall C st e v st' FUEL FUEL' (LE : FUEL <= FUEL'),
+    eval C st e FUEL = Resolved v st' ->
+    eval C st e FUEL' = Resolved v st'.
+Proof.
+  intros C st e v st' FUEL. revert C st e v st'.
+  induction FUEL; intros.
+  - inversion H.
+  - simpl in H; destruct e; inversion LE; eauto.
+    + remember (eval C st e1 FUEL) as v1.
+      destruct v1 as [ | | v1 st1]; inversion H.
+      clear H3. destruct v1 as [v1 | ]; inversion H.
+      clear H3. destruct v1 as [x v1 C_lam].
+      remember (eval C st1 e2 FUEL) as v2.
+      destruct v2 as [ | | v2 st2]; inversion H;
+      clear H3. destruct v2 as [v2 | ]; inversion H.
+      clear H3. destruct st2 as [mem2 t2].
+      remember (eval (C_lam [|dy_c_lam x t2 ([||])|]) 
+                     (ST (t2 :: dy_level C_lam !-> v2; mem2) (S t2))
+                      v1 FUEL) as v3.
+      destruct v3 as [ | | v3 st3]; inversion H.
+      clear H3. destruct v3 as [v3 | ]; inversion H.
+      subst.
+      assert (eval C st e1 m = Resolved (EVal (Closure x v1 C_lam)) st1) as RR1.
+      apply IHFUEL. nia. eauto.
+      assert (eval C st1 e2 m = Resolved (EVal v2) (ST mem2 t2)) as RR2.
+      apply IHFUEL. nia. eauto.
+      assert (eval (C_lam [|dy_c_lam x t2 ([||])|])
+                   (ST (t2 :: dy_level C_lam !-> v2; mem2) (S t2)) v1 m = 
+              Resolved (EVal v3) st') as RR3.
+      apply IHFUEL. nia. eauto.
+      simpl. rewrite RR1. rewrite RR2. rewrite RR3. eauto.
+    + remember (eval C st e1 FUEL) as v1.
+      destruct v1 as [ | | v1 st1]; inversion H.
+      clear H3. destruct v1 as [v1 | ]; inversion H.
+      remember (eval mv st1 e2 FUEL) as v2.
+      clear H3. destruct v2 as [ | | v2 st2]; inversion H.
+      clear H3. destruct v2 as [v2 | ]; inversion H. 
+      subst.
+      assert (eval C st e1 m = Resolved (MVal mv) st1) as RR1.
+      apply IHFUEL. nia. eauto.
+      assert (eval mv st1 e2 m = Resolved (EVal v2) st') as RR2.
+      apply IHFUEL. nia. eauto.
+      simpl. rewrite RR1. rewrite RR2. eauto.
+    + remember (eval C st e1 FUEL) as v1.
+      destruct v1 as [ | | v1 st1]; inversion H.
+      clear H3. destruct v1 as [v1 | ]; inversion H.
+      clear H3. destruct st1 as [mem1 t1].
+      remember (eval (C [|dy_c_lete x t1 ([||])|]) 
+                     (ST (t1 :: dy_level C !-> v1; mem1) (S t1))
+                      e2 FUEL) as v2.
+      destruct v2 as [ | | v2 st2]; inversion H.
+      clear H3. destruct v2 as [v2 | ]; inversion H.
+      subst.
+      assert (eval C st e1 m = Resolved (EVal v1) (ST mem1 t1)) as RR1.
+      apply IHFUEL. nia. eauto.
+      assert (eval (C [|dy_c_lete x t1 ([||])|]) 
+                   (ST (t1 :: dy_level C !-> v1; mem1) (S t1))
+                   e2 m = Resolved (MVal mv) st') as RR2.
+      apply IHFUEL. nia. eauto.
+      simpl. rewrite RR1. rewrite RR2. eauto.
+    + remember (eval C st e1 FUEL) as v1.
+      destruct v1 as [ | | v1 st1]; inversion H.
+      clear H3. destruct v1 as [v1 | ]; inversion H.
+      clear H3.
+      remember (eval (C [|dy_c_letm M mv ([||])|]) st1
+                      e2 FUEL) as v2.
+      destruct v2 as [ | | v2 st2]; inversion H.
+      clear H3. destruct v2 as [v2 | ]; inversion H.
+      subst.
+      assert (eval C st e1 m = Resolved (MVal mv) st1) as RR1.
+      apply IHFUEL. nia. eauto.
+      assert (eval (C [|dy_c_letm M mv ([||])|]) st1
+                   e2 m = Resolved (MVal mv0) st') as RR2.
+      apply IHFUEL. nia. eauto.
+      simpl. rewrite RR1. rewrite RR2. eauto.
+Qed.
+      
+Lemma EvalR_well_defined_l :
+  forall C st e v st' (R : EvalR C st e v st'),
+    exists FUEL, eval C st e FUEL = Resolved v st'.
+Proof.
+  intros. induction R.
+  - exists 1; simpl. 
+    remember (addr_x C x) as addr. destruct addr.
+    specialize (ADDR eq_refl). inversion ADDR.
+    rewrite <- STATE. rewrite <- ACCESS. eauto.
+  - exists 1; simpl; eauto.
+  - destruct IHR1 as [FUEL' EQ'].
+    destruct IHR2 as [FUEL'' EQ''].
+    destruct IHR3 as [FUEL''' EQ'''].
+    exists (S (Nat.max FUEL' (Nat.max FUEL'' FUEL'''))).
+    simpl.
+    assert (eval C st e1 (Nat.max FUEL' (Nat.max FUEL'' FUEL'''))
+            = Resolved (EVal (Closure x e C_lam)) st_lam) as RR.
+    apply relax_fuel with (FUEL := FUEL'). nia. eauto.
+    rewrite RR; clear RR.
+    assert (eval C st_lam e2 (Nat.max FUEL' (Nat.max FUEL'' FUEL'''))
+            = Resolved (EVal arg) (ST mem t)) as RR.
+    apply relax_fuel with (FUEL := FUEL''). nia. eauto.
+    rewrite RR; clear RR.
+    assert (eval (C_lam [|dy_c_lam x t ([||])|]) 
+                 (ST (t :: dy_level C_lam !-> arg; mem) (S t)) e
+                 (Nat.max FUEL' (Nat.max FUEL'' FUEL'''))
+            = Resolved (EVal v) st_v) as RR.
+    apply relax_fuel with (FUEL := FUEL'''). nia. eauto.
+    rewrite RR; clear RR. eauto.
+  - destruct IHR1 as [FUEL' EQ'].
+    destruct IHR2 as [FUEL'' EQ''].
+    exists (S (Nat.max FUEL' FUEL'')).
+    simpl.
+    assert (eval C st m (Nat.max FUEL' FUEL'')
+            = Resolved (MVal C_m) st_m) as RR.
+    apply relax_fuel with (FUEL := FUEL'). nia. eauto.
+    rewrite RR; clear RR.
+    assert (eval C_m st_m e (Nat.max FUEL' FUEL'')
+            = Resolved (EVal v) st_v) as RR.
+    apply relax_fuel with (FUEL := FUEL''). nia. eauto.
+    rewrite RR; clear RR. eauto. 
+  - exists 1. simpl; eauto. 
+  - exists 1; simpl. rewrite <- ACCESS. eauto. 
+  - destruct IHR1 as [FUEL' EQ'].
+    destruct IHR2 as [FUEL'' EQ''].
+    exists (S (Nat.max FUEL' FUEL'')).
+    simpl.
+    assert (eval C st e (Nat.max FUEL' FUEL'')
+            = Resolved (EVal v) (ST mem t)) as RR.
+    apply relax_fuel with (FUEL := FUEL'). nia. eauto.
+    rewrite RR; clear RR.
+    assert (eval (C [|dy_c_lete x t ([||])|]) 
+                 (ST (t :: dy_level C !-> v; mem) (S t)) m
+                 (Nat.max FUEL' FUEL'')
+            = Resolved (MVal C_m) st_m) as RR.
+    apply relax_fuel with (FUEL := FUEL''). nia. eauto.
+    rewrite RR; clear RR. eauto.
+  - destruct IHR1 as [FUEL' EQ'].
+    destruct IHR2 as [FUEL'' EQ''].
+    exists (S (Nat.max FUEL' FUEL'')).
+    simpl.
+    assert (eval C st m' (Nat.max FUEL' FUEL'')
+            = Resolved (MVal C') st') as RR.
+    apply relax_fuel with (FUEL := FUEL'). nia. eauto.
+    rewrite RR; clear RR.
+    assert (eval (C [|dy_c_letm M C' ([||])|]) st' m'' (Nat.max FUEL' FUEL'')
+            = Resolved (MVal C'') st'') as RR.
+    apply relax_fuel with (FUEL := FUEL''). nia. eauto.
+    rewrite RR; clear RR. eauto.
+Qed.
+
+Lemma EvalR_well_defined_r :
+  forall FUEL C st e v st' (R : eval C st e FUEL = Resolved v st'),
+    EvalR C st e v st'.
+Proof.
+  induction FUEL; intros; simpl in *; try (inversion R; fail).
+  destruct e.
+  - remember (addr_x C x) as addr. destruct addr.
+    inversion R. destruct st. 
+    remember (mem (t :: addr)) as access.
+    destruct access. inversion R. subst.
+    eapply Eval_var_e. eauto. rewrite <- Heqaddr. 
+    intro contra. inversion contra. rewrite <- Heqaddr. eauto.
+    inversion R.
+  - inversion R. eauto using EvalR.
+  - remember (eval C st e1 FUEL) as v1.
+    destruct v1 as [ | | v1 st1]; inversion R.
+    clear H0. destruct v1 as [v1 | ]; inversion R.
+    clear H0. destruct v1 as [x v1 C_lam].
+    remember (eval C st1 e2 FUEL) as v2.
+    destruct v2 as [ | | v2 st2]; inversion R.
+    clear H0. destruct v2 as [v2 | ]; inversion R.
+    clear H0. destruct st2 as [mem2 t2].
+    remember (eval (C_lam [|dy_c_lam x t2 ([||])|])
+                   (ST (t2 :: dy_level C_lam !-> v2; mem2) (S t2)) 
+                   v1 FUEL) as v3.
+    destruct v3 as [ | | v3 st3]; inversion R.
+    clear H0. destruct v3 as [v3 | ]; inversion R.
+    subst.
+    assert (EvalR C st e1 (EVal (Closure x v1 C_lam)) st1) as RR1. eauto.
+    assert (EvalR C st1 e2 (EVal v2) (ST mem2 t2)) as RR2. eauto.
+    assert (EvalR (C_lam [|dy_c_lam x t2 ([||])|])
+                  (ST (t2 :: dy_level C_lam !-> v2; mem2) (S t2)) v1
+            (EVal v3) st') as RR3. eauto.
+    eauto using EvalR.
+  - remember (eval C st e1 FUEL) as v1.
+    destruct v1 as [ | | v1 st1]; inversion R.
+    clear H0. destruct v1 as [v1 | ]; inversion R.
+    clear H0. remember (eval mv st1 e2 FUEL) as v2.
+    destruct v2 as [ | | v2 st2]; inversion R.
+    clear H0. destruct v2 as [v2 | ]; inversion R.
+    subst.
+    eauto using EvalR.
+  - inversion R; subst. eauto using EvalR.
+  - remember (ctx_M C M) as ACCESS.
+    destruct ACCESS; inversion R; subst.
+    eauto using EvalR.
+  - remember (eval C st e1 FUEL) as v1.
+    destruct v1 as [ | | v1 st1]; inversion R.
+    clear H0. destruct v1 as [v1 | ]; inversion R.
+    clear H0. destruct st1 as [mem1 t1].
+    remember (eval (C [|dy_c_lete x t1 ([||])|])
+                   (ST (t1 :: dy_level C !-> v1; mem1) (S t1)) 
+                   e2 FUEL) as v2.
+    destruct v2 as [ | | v2 st2]; inversion R.
+    clear H0. destruct v2 as [v2 | ]; inversion R.
+    subst.
+    assert (EvalR C st e1 (EVal v1) (ST mem1 t1)) as RR1. eauto.
+    assert (EvalR (C [|dy_c_lete x t1 ([||])|])
+                  (ST (t1 :: dy_level C !-> v1; mem1) (S t1)) e2
+            (MVal mv) st') as RR2. eauto.
+    eauto using EvalR.
+  - remember (eval C st e1 FUEL) as v1.
+    destruct v1 as [ | | v1 st1]; inversion R.
+    clear H0. destruct v1 as [v1 | ]; inversion R.
+    clear H0.
+    remember (eval (C [|dy_c_letm M mv ([||])|]) st1 e2 FUEL) as v2.
+    destruct v2 as [ | | v2 st2]; inversion R.
+    clear H0. destruct v2 as [v2 | ]; inversion R.
+    subst.
+    assert (EvalR C st e1 (MVal mv) st1) as RR1. eauto.
+    assert (EvalR (C [|dy_c_letm M mv ([||])|])
+                  st1 e2 (MVal mv0) st') as RR2. eauto.
+    eauto using EvalR.
+Qed.
+
+Theorem EvalR_well_defined :
+  forall C st e v st',
+    (exists FUEL, eval C st e FUEL = Resolved v st') <->
+    EvalR C st e v st'.
+Proof.
+  intros; split; try apply EvalR_well_defined_l.
+  intros. destruct H as [FUEL EVAL].
+  eapply EvalR_well_defined_r. eauto.
+Qed.
 
 Definition Reach (tm1 tm2 : Type) := tm1 -> dy_ctx -> state -> tm2 -> Prop.
 
-(* Reachability relation, sensible version *)
-Inductive _EreachE (C : dy_ctx) (st : state)
-    : Reach expr_tm expr_tm :=
-  | _ere_refl e
-    : _EreachE C st e 
-               C st e
-  | _ere_var x mem t v pf C_v
-            (STATE : ST mem t = st)
-            (ADDR : [] <> addr_x C x)
-            (ACCESS : Some (Val v pf C_v) = mem (addr_x C x))
-    : _EreachE C st (e_var x) 
-               C_v st v
-  | _ere_app_left e1 e2 C' st' e'
-                 (REACHl : _EreachE C st e1
-                                    C' st' e')
-    : _EreachE C st (e_app e1 e2) 
-               C' st' e'
-  | _ere_app_right e1 e2 st1 v C' st' e'
-                  (FN : EevalR C st e1 v st1)
-                  (REACHr : _EreachE C st1 e2
-                                     C' st' e')
-    : _EreachE C st (e_app e1 e2)
-               C' st' e'
-  | _ere_app_body e1 e2 x e C_lam st_lam
-                 arg mem t
-                 C' st' e'
-                 (FN : EevalR C st e1 
-                             (Val (e_lam x e) (v_fn x e) C_lam) st_lam)
-                 (ARG : EevalR C st_lam e2
-                               arg (ST mem t))
-                 (REACHb : _EreachE (C_lam[|dy_c_lam x t  ([||])|]) 
-                                    (ST (t :: (dy_level C_lam) !-> arg ; mem) (update_t t)) e
-                                     C' st' e')
-    : _EreachE C st (e_app e1 e2)
-               C' st' e'
-  | _ere_link_m m e C' st' e'
-               (REACHm : _MreachE C st m
-                                  C' st' e')
-    : _EreachE C st (e_link m e)
-               C' st' e'
-  | _ere_link_e m e C_m st_m C' st' e'
-               (MOD : MevalR C st m C_m st_m)
-               (REACHe : _EreachE C_m st_m e
-                                  C' st' e')
-    : _EreachE C st (e_link m e)
-               C' st' e'
-
-with _MreachE (C : dy_ctx) (st : state)
-    : Reach mod_tm expr_tm :=
-  | _mre_lete_e x e m C' st' e'
-               (REACHe : _EreachE C st e
-                                  C' st' e')
-    : _MreachE C st (m_lete x e m)
-               C' st' e'
-  | _mre_lete_m x e m v mem t
+(* Reachability relation *)
+Inductive ReachR (C : dy_ctx) (st : state)
+    : Reach tm tm :=
+  | r_refl e
+    : ReachR C st e 
+             C st e
+  | r_app_left e1 e2 C' st' e'
+               (REACHl : ReachR C st e1
+                                C' st' e')
+    : ReachR C st (e_app e1 e2) 
+             C' st' e'
+  | r_app_right e1 e2 x e C_lam st_lam C' st' e'
+                (FN : EvalR C st e1 
+                            (EVal (Closure x e C_lam)) st_lam)
+                (REACHr : ReachR C st_lam e2
+                                 C' st' e')
+    : ReachR C st (e_app e1 e2)
+             C' st' e'
+  | r_app_body e1 e2 x e C_lam st_lam
+                arg mem t
                 C' st' e'
-             (EVALx : EevalR C st e v (ST mem t))
-             (REACHm : _MreachE (C[|dy_c_lete x t  ([||])|])
-                                (ST (t :: (dy_level C) !-> v ; mem) (update_t t)) m
+                (FN : EvalR C st e1 
+                            (EVal (Closure x e C_lam)) st_lam)
+                (ARG : EvalR C st_lam e2
+                             (EVal arg) (ST mem t))
+                (REACHb : ReachR (C_lam[|dy_c_lam x t ([||])|]) 
+                                 (ST (t :: (dy_level C_lam) !-> arg ; mem) 
+                                     (update_t C (ST mem t) x arg)) e
                                  C' st' e')
-    : _MreachE C st (m_lete x e m)
-               C' st' e'
-  | _mre_letm_m1 M m1 m2 C' st' e'
-               (REACHm : _MreachE C st m1
-                                  C' st' e')
-    : _MreachE C st (m_letm M m1 m2)
-               C' st' e'
-  | _mre_letm_m2 M m1 m2 C_M st_M
-                 C' st' e'
-             (EVALM : MevalR C st m1 C_M st_M)
-             (REACHm : _MreachE (C[|dy_c_letm M C_M ([||])|]) st_M m2
-                                 C' st' e')
-    : _MreachE C st (m_letm M m1 m2)
-               C' st' e'.
-
-Scheme __EreachE_ind_mut := Induction for _EreachE Sort Prop
-with __MreachE_ind_mut := Induction for _MreachE Sort Prop.
-
-Inductive _MreachM (C : dy_ctx) (st : state)
-    : Reach mod_tm mod_tm :=
-  | _mrm_refl m
-    : _MreachM C st m
-               C st m
-  | _mrm_var M C_M (ACCESS : Some C_M = ctx_M C M)
-    : _MreachM C st (m_var M)
-               C_M st m_empty
-  | _mrm_lete_e x e m C' st' m'
-               (REACHe : _EreachM C st e
-                                  C' st' m')
-    : _MreachM C st (m_lete x e m)
-               C' st' m'
-  | _mrm_lete_m x e m v mem t
-                C' st' m'
-             (EVALx : EevalR C st e v (ST mem t))
-             (REACHm : _MreachM (C[|dy_c_lete x t  ([||])|]) 
-                                (ST (t :: (dy_level C) !-> v ; mem) (update_t t)) m
-                                 C' st' m')
-    : _MreachM C st (m_lete x e m)
-               C' st' m'
-  | _mrm_letm_m1 M m1 m2 C' st' m'
-               (REACHm : _MreachM C st m1
-                                  C' st' m')
-    : _MreachM C st (m_letm M m1 m2)
-               C' st' m'
-  | _mrm_letm_m2 M m1 m2 C_M st_M
-                 C' st' m'
-             (EVALM : MevalR C st m1 C_M st_M)
-             (REACHm : _MreachM (C[|dy_c_letm M C_M ([||])|]) st_M m2
-                                 C' st' m')
-    : _MreachM C st (m_letm M m1 m2)
-               C' st' m'
-
-with _EreachM (C : dy_ctx) (st : state)
-    : Reach expr_tm mod_tm :=
-  | _erm_app_left e1 e2 C' st' m'
-                 (REACHl : _EreachM C st e1
-                                    C' st' m')
-    : _EreachM C st (e_app e1 e2) 
-               C' st' m'
-  | _erm_app_right e1 e2 v1 st1 C' st' m'
-                  (FN : EevalR C st e1 v1 st1)
-                  (REACHr : _EreachM C st1 e2
-                                     C' st' m')
-    : _EreachM C st (e_app e1 e2)
-               C' st' m'
-  | _erm_app_body e1 e2 x e C_lam st_lam
-                 arg mem t
-                 C' st' m'
-                 (FN : EevalR C st e1 
-                              (Val (e_lam x e) (v_fn x e) C_lam) st_lam)
-                 (ARG : EevalR C st_lam e2 arg (ST mem t))
-                 (REACHb : _EreachM (C_lam[|dy_c_lam x t ([||])|]) 
-                                    (ST (t :: (dy_level C_lam) !-> arg ; mem) (update_t t)) e
-                                     C' st' m')
-    : _EreachM C st (e_app e1 e2)
-               C' st' m'
-  | _erm_link_m m e C' st' m'
-               (REACHm : _MreachM C st m
-                                  C' st' m')
-    : _EreachM C st (e_link m e)
-               C' st' m'
-  | _erm_link_e m e C_m st_m C' st' m'
-               (MOD : MevalR C st m C_m st_m)
-               (REACHe : _EreachM C_m st_m e
-                                  C' st' m')
-    : _EreachM C st (e_link m e)
-               C' st' m'
+    : ReachR C st (e_app e1 e2)
+             C' st' e'
+  | r_link_m m e C' st' e'
+              (REACHm : ReachR C st m
+                               C' st' e')
+    : ReachR C st (e_link m e)
+             C' st' e'
+  | r_link_e m e C_m st_m C' st' e'
+             (MOD : EvalR C st m (MVal C_m) st_m)
+             (REACHe : ReachR C_m st_m e
+                              C' st' e')
+    : ReachR C st (e_link m e)
+             C' st' e'
+  | r_lete_e x e m C' st' e'
+             (REACHe : ReachR C st e
+                              C' st' e')
+    : ReachR C st (m_lete x e m)
+             C' st' e'
+  | r_lete_m x e m v mem t
+             C' st' e'
+             (EVALx : EvalR C st e (EVal v) (ST mem t))
+             (REACHm : ReachR (C[|dy_c_lete x t ([||])|])
+                              (ST (t :: (dy_level C) !-> v ; mem) 
+                                  (update_t C (ST mem t) x v)) m
+                              C' st' e')
+    : ReachR C st (m_lete x e m)
+             C' st' e'
+  | r_letm_m1 M m1 m2 C' st' e'
+              (REACHm : ReachR C st m1
+                               C' st' e')
+    : ReachR C st (m_letm M m1 m2)
+             C' st' e'
+  | r_letm_m2 M m1 m2 C_M st_M
+              C' st' e'
+              (EVALM : EvalR C st m1 (MVal C_M) st_M)
+              (REACHm : ReachR (C[|dy_c_letm M C_M ([||])|]) st_M m2
+                               C' st' e')
+    : ReachR C st (m_letm M m1 m2)
+             C' st' e'
 .
 
-Scheme __EreachM_ind_mut := Induction for _EreachM Sort Prop
-with __MreachM_ind_mut := Induction for _MreachM Sort Prop.
-
-(* for proofs *)
-Inductive EreachE (C : dy_ctx) (st : state)
-    : Reach expr_tm expr_tm :=
-  | ere_refl e
-    : EreachE C st e 
-              C st e
-  | ere_var x mem t v pf C_v
-            (STATE : ST mem t = st)
-            (ADDR : [] <> addr_x C x)
-            (ACCESS : Some (Val v pf C_v) = mem (addr_x C x))
-    : EreachE C st (e_var x) 
-              C_v st v
-  | ere_app_left e1 e2 C' st' e'
-                 (REACHl : EreachE C st e1
-                                   C' st' e')
-    : EreachE C st (e_app e1 e2) 
-              C' st' e'
-  | ere_app_right e1 e2 st_lam v pf C_lam C' st' e'
-                  (FN : EevalR C st e1 (Val v pf C_lam) st_lam)
-                  (FNr : EreachE C st e1 C_lam st_lam v)
-                  (REACHr : EreachE C st_lam e2
-                                    C' st' e')
-    : EreachE C st (e_app e1 e2)
-              C' st' e'
-  | ere_app_body e1 e2 x e C_lam st_lam
-                 arg pf C_arg mem t
-                 C' st' e'
-                 (FN : EevalR C st e1 
-                             (Val (e_lam x e) (v_fn x e) C_lam) st_lam)
-                 (FNr : EreachE C st e1 C_lam st_lam (e_lam x e))
-                 (ARG : EevalR C st_lam e2
-                               (Val arg pf C_arg) (ST mem t))
-                 (ARGr : EreachE C st_lam e2 C_arg (ST mem t) arg)
-                 (REACHb : EreachE (C_lam[|dy_c_lam x t ([||])|]) 
-                                    (ST (t :: (dy_level C_lam) !-> (Val arg pf C_arg) ; mem) (update_t t)) e
-                                     C' st' e')
-    : EreachE C st (e_app e1 e2)
-              C' st' e'
-  | ere_link_m m e C' st' e'
-               (REACHm : MreachE C st m
-                                 C' st' e')
-    : EreachE C st (e_link m e)
-              C' st' e'
-  | ere_link_e m e C_m st_m C' st' e'
-              (MOD : MevalR C st m C_m st_m)
-              (MODr : MreachM C st m C_m st_m m_empty)
-              (REACHe : EreachE C_m st_m e
-                                C' st' e')
-    : EreachE C st (e_link m e)
-              C' st' e'
-
-with MreachE (C : dy_ctx) (st : state)
-    : Reach mod_tm expr_tm :=
-  | mre_lete_e x e m C' st' e'
-               (REACHe : EreachE C st e
-                                 C' st' e')
-    : MreachE C st (m_lete x e m)
-              C' st' e'
-  | mre_lete_m x e m v pf C_x mem t
-               C' st' e'
-             (EVALx : EevalR C st e (Val v pf C_x) (ST mem t))
-             (EVALxr : EreachE C st e C_x (ST mem t) v)
-             (REACHm : MreachE (C[|dy_c_lete x t ([||])|])
-                                (ST (t :: (dy_level C) !-> (Val v pf C_x) ; mem) (update_t t)) m
-                                 C' st' e')
-    : MreachE C st (m_lete x e m)
-              C' st' e'
-  | mre_letm_m1 M m1 m2 C' st' e'
-              (REACHm : MreachE C st m1
-                                C' st' e')
-    : MreachE C st (m_letm M m1 m2)
-              C' st' e'
-  | mre_letm_m2 M m1 m2 C_M st_M
-                C' st' e'
-             (EVALM : MevalR C st m1 C_M st_M)
-             (EVALM : MreachM C st m1 C_M st_M m_empty)
-             (REACHm : MreachE (C[|dy_c_letm M C_M ([||])|]) st_M m2
-                                C' st' e')
-    : MreachE C st (m_letm M m1 m2)
-              C' st' e'
-
-with MreachM (C : dy_ctx) (st : state)
-    : Reach mod_tm mod_tm :=
-  | mrm_refl m
-    : MreachM C st m
-              C st m
-  | mrm_var M C_M (ACCESS : Some C_M = ctx_M C M)
-    : MreachM C st (m_var M)
-              C_M st m_empty
-  | mrm_lete_e x e m C' st' m'
-               (REACHe : EreachM C st e
-                                  C' st' m')
-    : MreachM C st (m_lete x e m)
-              C' st' m'
-  | mrm_lete_m x e m v pf C_x mem t
-               C' st' m'
-             (EVALx : EevalR C st e (Val v pf C_x) (ST mem t))
-             (EVALxr : EreachE C st e C_x (ST mem t) v)
-             (REACHm : MreachM (C[|dy_c_lete x t ([||])|]) 
-                               (ST (t :: (dy_level C) !-> (Val v pf C_x) ; mem) (update_t t)) m
-                                C' st' m')
-    : MreachM C st (m_lete x e m)
-              C' st' m'
-  | mrm_letm_m1 M m1 m2 C' st' m'
-               (REACHm : MreachM C st m1
-                                 C' st' m')
-    : MreachM C st (m_letm M m1 m2)
-              C' st' m'
-  | mrm_letm_m2 M m1 m2 C_M st_M
-                C' st' m'
-             (EVALM : MevalR C st m1 C_M st_M)
-             (EVALMr : MreachM C st m1 C_M st_M m_empty)
-             (REACHm : MreachM (C[|dy_c_letm M C_M ([||])|]) st_M m2
-                                C' st' m')
-    : MreachM C st (m_letm M m1 m2)
-              C' st' m'
-
-with EreachM (C : dy_ctx) (st : state)
-    : Reach expr_tm mod_tm :=
-  | erm_app_left e1 e2 C' st' m'
-                (REACHl : EreachM C st e1
-                                  C' st' m')
-    : EreachM C st (e_app e1 e2) 
-              C' st' m'
-  | erm_app_right e1 e2 v pf C_lam st_lam C' st' m'
-                 (FN : EevalR C st e1 (Val v pf C_lam) st_lam)
-                 (FNr : EreachE C st e1 C_lam st_lam v)
-                 (REACHr : EreachM C st_lam e2
-                                   C' st' m')
-    : EreachM C st (e_app e1 e2)
-              C' st' m'
-  | erm_app_body e1 e2 x e C_lam st_lam
-                 arg pf C_arg mem t
-                 C' st' m'
-                 (FN : EevalR C st e1 
-                              (Val (e_lam x e) (v_fn x e) C_lam) st_lam)
-                 (FNr : EreachE C st e1 
-                                C_lam st_lam (e_lam x e))
-                 (ARG : EevalR C st_lam e2 (Val arg pf C_arg) (ST mem t))
-                 (ARGr : EreachE C st_lam e2 C_arg (ST mem t) arg)
-                 (REACHb : EreachM (C_lam[|dy_c_lam x t ([||])|]) 
-                                   (ST (t :: (dy_level C_lam) !-> (Val arg pf C_arg) ; mem) (update_t t)) e
-                                    C' st' m')
-    : EreachM C st (e_app e1 e2)
-              C' st' m'
-  | erm_link_m m e C' st' m'
-              (REACHm : MreachM C st m
-                                C' st' m')
-    : EreachM C st (e_link m e)
-              C' st' m'
-  | erm_link_e m e C_m st_m C' st' m'
-              (MOD : MevalR C st m C_m st_m)
-              (MODr : MreachM C st m C_m st_m m_empty)
-              (REACHe : EreachM C_m st_m e
-                                C' st' m')
-    : EreachM C st (e_link m e)
-              C' st' m'
-.
-
-Scheme _EreachE_ind_mut := Induction for EreachE Sort Prop
-with _EreachM_ind_mut := Induction for EreachM Sort Prop
-with _MreachE_ind_mut := Induction for MreachE Sort Prop
-with _MreachM_ind_mut := Induction for MreachM Sort Prop.
-
-Notation "'<e|' C1 st1 tm1 '~>' C2 st2 tm2 '|e>'" := (EreachE C1 st1 tm1 C2 st2 tm2) 
-                                               (at level 10, 
-                                                C1 at next level, st1 at next level, tm1 at next level,
-                                                C2 at next level, st2 at next level, tm2 at next level).
-
-Notation "'<m|' C1 st1 tm1 '~>' C2 st2 tm2 '|e>'" := (MreachE C1 st1 tm1 C2 st2 tm2) 
-                                               (at level 10, 
-                                                C1 at next level, st1 at next level, tm1 at next level,
-                                                C2 at next level, st2 at next level, tm2 at next level).
-
-Notation "'<m|' C1 st1 tm1 '~>' C2 st2 tm2 '|m>'" := (MreachM C1 st1 tm1 C2 st2 tm2) 
-                                               (at level 10, 
-                                                C1 at next level, st1 at next level, tm1 at next level,
-                                                C2 at next level, st2 at next level, tm2 at next level).
-
-Notation "'<e|' C1 st1 tm1 '~>' C2 st2 tm2 '|m>'" := (EreachM C1 st1 tm1 C2 st2 tm2) 
+Notation "'<|' C1 st1 tm1 '~>' C2 st2 tm2 '|>'" := (ReachR C1 st1 tm1 C2 st2 tm2) 
                                                (at level 10, 
                                                 C1 at next level, st1 at next level, tm1 at next level,
                                                 C2 at next level, st2 at next level, tm2 at next level).
 
 (* sanity check *)
-Lemma ere_trans : forall C1 st1 e1
+Lemma reach_trans : forall C1 st1 e1
                          C2 st2 e2
                          C3 st3 e3
-                         (REACH1 : <e| C1 st1 e1 ~> C2 st2 e2 |e>)
-                         (REACH2 : <e| C2 st2 e2 ~> C3 st3 e3 |e>),
-                         <e| C1 st1 e1 ~> C3 st3 e3 |e>.
+                         (REACH1 : <| C1 st1 e1 ~> C2 st2 e2 |>)
+                         (REACH2 : <| C2 st2 e2 ~> C3 st3 e3 |>),
+                         <| C1 st1 e1 ~> C3 st3 e3 |>.
 Proof.
   intros. generalize dependent e3.
   revert C3 st3.
-  apply (_EreachE_ind_mut
-    (fun C1 st1 e1 
-         C2 st2 e2 
-         (REACH1 : <e| C1 st1 e1 ~> C2 st2 e2 |e>)=> 
-         forall C3 st3 e3 
-                (REACH2 : <e| C2 st2 e2 ~> C3 st3 e3 |e>),
-                <e| C1 st1 e1 ~> C3 st3 e3 |e>)
-    (fun C1 st1 e1 
-         C2 st2 m2 
-         (REACH1 : <e| C1 st1 e1 ~> C2 st2 m2 |m>)=> 
-         forall C3 st3 e3 
-                (REACH2 : <m| C2 st2 m2 ~> C3 st3 e3 |e>),
-                <e| C1 st1 e1 ~> C3 st3 e3 |e>)
-    (fun C1 st1 m1
-         C2 st2 e2
-         (REACH1 : <m| C1 st1 m1 ~> C2 st2 e2 |e>) =>
-         forall C3 st3 e3 
-                (REACH2 : <e| C2 st2 e2 ~> C3 st3 e3 |e>),
-                <m| C1 st1 m1 ~> C3 st3 e3 |e>)
-    (fun C1 st1 m1 
-         C2 st2 m2 
-         (REACH1 : <m| C1 st1 m1 ~> C2 st2 m2 |m>)=> 
-         forall C3 st3 e3 
-                (REACH2 : <m| C2 st2 m2 ~> C3 st3 e3 |e>),
-                <m| C1 st1 m1 ~> C3 st3 e3 |e>));
-   eauto using EreachE, EreachM, MreachE, MreachM;
-   intros; try inversion pf; subst; inversion REACH2; subst;
-   eauto using EreachE, EreachM, MreachE, MreachM.
-Qed.
-
-Lemma mrm_trans : forall C1 st1 m1
-                         C2 st2 m2
-                         C3 st3 m3
-                         (REACH1 : <m| C1 st1 m1 ~> C2 st2 m2 |m>)
-                         (REACH2 : <m| C2 st2 m2 ~> C3 st3 m3 |m>),
-                         <m| C1 st1 m1 ~> C3 st3 m3 |m>.
-Proof.
-  intros. generalize dependent m3.
-  revert C3 st3.
-  apply (_MreachM_ind_mut
-    (fun C1 st1 e1 
-         C2 st2 e2 
-         (REACH1 : <e| C1 st1 e1 ~> C2 st2 e2 |e>)=> 
-         forall C3 st3 m3 
-                (REACH2 : <e| C2 st2 e2 ~> C3 st3 m3 |m>),
-                <e| C1 st1 e1 ~> C3 st3 m3 |m>)
-    (fun C1 st1 e1 
-         C2 st2 m2 
-         (REACH1 : <e| C1 st1 e1 ~> C2 st2 m2 |m>)=> 
-         forall C3 st3 m3 
-                (REACH2 : <m| C2 st2 m2 ~> C3 st3 m3 |m>),
-                <e| C1 st1 e1 ~> C3 st3 m3 |m>)
-    (fun C1 st1 m1
-         C2 st2 e2
-         (REACH1 : <m| C1 st1 m1 ~> C2 st2 e2 |e>) =>
-         forall C3 st3 m3 
-                (REACH2 : <e| C2 st2 e2 ~> C3 st3 m3 |m>),
-                <m| C1 st1 m1 ~> C3 st3 m3 |m>)
-    (fun C1 st1 m1 
-         C2 st2 m2 
-         (REACH1 : <m| C1 st1 m1 ~> C2 st2 m2 |m>)=> 
-         forall C3 st3 m3 
-                (REACH2 : <m| C2 st2 m2 ~> C3 st3 m3 |m>),
-                <m| C1 st1 m1 ~> C3 st3 m3 |m>));
-   eauto using EreachE, EreachM, MreachE, MreachM;
-   intros; try inversion pf; subst; inversion REACH2; subst;
-   eauto using EreachE, EreachM, MreachE, MreachM.
-Qed.
-
-Lemma ermre_trans : forall C1 st1 e1
-                           C2 st2 m2
-                           C3 st3 e3
-                           (REACH1 : <e| C1 st1 e1 ~> C2 st2 m2 |m>)
-                           (REACH2 : <m| C2 st2 m2 ~> C3 st3 e3 |e>),
-                           <e| C1 st1 e1 ~> C3 st3 e3 |e>. 
-Proof.
-  intros. generalize dependent e3.
-  revert C3 st3.
-  apply (_EreachM_ind_mut
-    (fun C1 st1 e1 
-         C2 st2 e2 
-         (REACH1 : <e| C1 st1 e1 ~> C2 st2 e2 |e>)=> 
-         forall C3 st3 e3 
-                (REACH2 : <e| C2 st2 e2 ~> C3 st3 e3 |e>),
-                <e| C1 st1 e1 ~> C3 st3 e3 |e>)
-    (fun C1 st1 e1 
-         C2 st2 m2 
-         (REACH1 : <e| C1 st1 e1 ~> C2 st2 m2 |m>)=> 
-         forall C3 st3 e3 
-                (REACH2 : <m| C2 st2 m2 ~> C3 st3 e3 |e>),
-                <e| C1 st1 e1 ~> C3 st3 e3 |e>)
-    (fun C1 st1 m1
-         C2 st2 e2
-         (REACH1 : <m| C1 st1 m1 ~> C2 st2 e2 |e>) =>
-         forall C3 st3 e3 
-                (REACH2 : <e| C2 st2 e2 ~> C3 st3 e3 |e>),
-                <m| C1 st1 m1 ~> C3 st3 e3 |e>)
-    (fun C1 st1 m1 
-         C2 st2 m2 
-         (REACH1 : <m| C1 st1 m1 ~> C2 st2 m2 |m>)=> 
-         forall C3 st3 e3 
-                (REACH2 : <m| C2 st2 m2 ~> C3 st3 e3 |e>),
-                <m| C1 st1 m1 ~> C3 st3 e3 |e>));
-   eauto using EreachE, EreachM, MreachE, MreachM;
-   intros; try inversion pf; subst; inversion REACH2; subst;
-   eauto using EreachE, EreachM, MreachE, MreachM.
-Qed.
-
-Lemma mrerm_trans : forall C1 st1 m1
-                           C2 st2 e2
-                           C3 st3 m3
-                           (REACH1 : <m| C1 st1 m1 ~> C2 st2 e2 |e>)
-                           (REACH2 : <e| C2 st2 e2 ~> C3 st3 m3 |m>),
-                           <m| C1 st1 m1 ~> C3 st3 m3 |m>. 
-Proof.
-  intros. generalize dependent m3.
-  revert C3 st3.
-  apply (_MreachE_ind_mut
-    (fun C1 st1 e1 
-         C2 st2 e2 
-         (REACH1 : <e| C1 st1 e1 ~> C2 st2 e2 |e>)=> 
-         forall C3 st3 m3 
-                (REACH2 : <e| C2 st2 e2 ~> C3 st3 m3 |m>),
-                <e| C1 st1 e1 ~> C3 st3 m3 |m>)
-    (fun C1 st1 e1 
-         C2 st2 m2 
-         (REACH1 : <e| C1 st1 e1 ~> C2 st2 m2 |m>)=> 
-         forall C3 st3 m3 
-                (REACH2 : <m| C2 st2 m2 ~> C3 st3 m3 |m>),
-                <e| C1 st1 e1 ~> C3 st3 m3 |m>)
-    (fun C1 st1 m1
-         C2 st2 e2
-         (REACH1 : <m| C1 st1 m1 ~> C2 st2 e2 |e>) =>
-         forall C3 st3 m3 
-                (REACH2 : <e| C2 st2 e2 ~> C3 st3 m3 |m>),
-                <m| C1 st1 m1 ~> C3 st3 m3 |m>)
-    (fun C1 st1 m1 
-         C2 st2 m2 
-         (REACH1 : <m| C1 st1 m1 ~> C2 st2 m2 |m>)=> 
-         forall C3 st3 m3 
-                (REACH2 : <m| C2 st2 m2 ~> C3 st3 m3 |m>),
-                <m| C1 st1 m1 ~> C3 st3 m3 |m>));
-   eauto using EreachE, EreachM, MreachE, MreachM;
-   intros; try inversion pf; subst; inversion REACH2; subst;
-   eauto using EreachE, EreachM, MreachE, MreachM.
+  induction REACH1; eauto using ReachR.
 Qed.
 
 Lemma c_plugin_assoc : forall C1 C2 C3, C1[| C2[| C3 |] |] = ((C1[|C2|])[|C3|]).
@@ -713,106 +602,6 @@ Proof.
   eauto; try apply eq_p_eq; eauto;
   specialize (IHC1 C2); rewrite eq_p_eq in IHC1;
   rewrite IHC1; rewrite app_assoc; eauto.
-Qed.
-
-(* equivalence between reachability relations *)
-Lemma Eeval_then_reach :
-    forall Ci sti ei v stv
-           (EVAL : EevalR Ci sti ei v stv)
-           ev pf Cv mem t
-           (VAL : v = Val ev pf Cv)
-           (STATE : stv = ST mem t),
-          <e| Ci sti ei ~> Cv stv ev |e>.
-Proof.
-  apply (EevalR_ind_mut
-    (fun Ci sti ei v stv
-        (EVAL : EevalR Ci sti ei v stv) =>
-        forall ev pf Cv mem t
-              (VAL : v = Val ev pf Cv)
-              (STATE : stv = ST mem t),
-        <e| Ci sti ei ~> Cv stv ev |e>)
-    (fun Ci sti mi Cv stv
-        (EVAL : MevalR Ci sti mi Cv stv) =>
-        <m| Ci sti mi ~> Cv stv m_empty |m>));
-  intros; try inversion STATE0; try inversion STATE;
-          try inversion VAL; try destruct st_lam;
-          try destruct st_m; try destruct v_e;
-          try destruct v_m1; try destruct arg; subst; 
-          eauto using EreachE, EreachM, MreachE, MreachM.
-Qed.
-
-Lemma Meval_then_reach :
-    forall Ci sti mi Cv stv
-           (EVAL : MevalR Ci sti mi Cv stv),
-           <m| Ci sti mi ~> Cv stv m_empty |m>.
-Proof.
-  apply (MevalR_ind_mut
-    (fun Ci sti ei v stv
-        (EVAL : EevalR Ci sti ei v stv) =>
-        forall ev pf Cv mem t
-              (VAL : v = Val ev pf Cv)
-              (STATE : stv = ST mem t),
-        <e| Ci sti ei ~> Cv stv ev |e>)
-    (fun Ci sti mi Cv stv
-        (EVAL : MevalR Ci sti mi Cv stv) =>
-        <m| Ci sti mi ~> Cv stv m_empty |m>));
-  intros; try inversion STATE0; try inversion STATE;
-          try inversion VAL; try destruct st_lam;
-          try destruct st_m; try destruct v_e;
-          try destruct v_m1; try destruct arg; subst; 
-          eauto using EreachE, EreachM, MreachE, MreachM.
-Qed.
-
-Lemma EreachE_equiv_left :
-    forall C1 st1 e1 C2 st2 e2,
-          <e| C1 st1 e1 ~> C2 st2 e2 |e> ->
-          _EreachE C1 st1 e1 C2 st2 e2.
-Proof.
-  apply (_EreachE_ind_mut 
-    (fun C1 st1 e1 C2 st2 e2
-        (REACH : <e| C1 st1 e1 ~> C2 st2 e2 |e>) =>
-        _EreachE C1 st1 e1 C2 st2 e2)
-    (fun C1 st1 e1 C2 st2 m2
-        (REACH : <e| C1 st1 e1 ~> C2 st2 m2 |m>) =>
-        _EreachM C1 st1 e1 C2 st2 m2)
-    (fun C1 st1 m1 C2 st2 e2
-        (REACH : <m| C1 st1 m1 ~> C2 st2 e2 |e>) =>
-        _MreachE C1 st1 m1 C2 st2 e2)
-    (fun C1 st1 m1 C2 st2 m2
-        (REACH : <m| C1 st1 m1 ~> C2 st2 m2 |m>) =>
-        _MreachM C1 st1 m1 C2 st2 m2));
-  intros; eauto using EreachE, EreachM, MreachE, MreachM, _EreachE, _MreachE, _EreachM, _MreachM.
-Qed.
-
-Lemma EreachE_equiv_right :
-    forall C1 st1 e1 C2 st2 e2,
-          _EreachE C1 st1 e1 C2 st2 e2 ->
-          <e| C1 st1 e1 ~> C2 st2 e2 |e>.
-Proof.
-  apply (__EreachE_ind_mut 
-    (fun C1 st1 e1 C2 st2 e2
-        (REACH : _EreachE C1 st1 e1 C2 st2 e2) =>
-        <e| C1 st1 e1 ~> C2 st2 e2 |e>)
-    (fun C1 st1 m1 C2 st2 e2
-        (REACH : _MreachE C1 st1 m1 C2 st2 e2) =>
-        <m| C1 st1 m1 ~> C2 st2 e2 |e>));
-  intros; try destruct v; try destruct st; try destruct st1; try destruct st_lam;
-  try destruct arg; try destruct st_m; try destruct st';
-  eauto using EreachE, EreachM, MreachE, MreachM, _EreachE, _MreachE, _EreachM, _MreachM.
-  - eapply Eeval_then_reach in FN as FNr; eauto using EreachE.
-  - eapply Eeval_then_reach in FN as FNr; eauto using EreachE.
-    eapply Eeval_then_reach in ARG as ARGr; eauto using EreachE.
-  - eapply Meval_then_reach in MOD as MODr; eauto using EreachE.
-  - eapply Eeval_then_reach in EVALx as EVALxr; eauto using MreachE.
-  - eapply Meval_then_reach in EVALM as EVALMr; eauto using MreachE.
-Qed.
-
-Theorem EreachE_equiv : 
-  forall C1 st1 e1 C2 st2 e2,
-         _EreachE C1 st1 e1 C2 st2 e2 <->
-          <e| C1 st1 e1 ~> C2 st2 e2 |e>.
-Proof. 
-  intros; split; try apply EreachE_equiv_left; try apply EreachE_equiv_right. 
 Qed.
 
 Fixpoint dy_to_st C :=
@@ -868,226 +657,41 @@ Proof.
       exists dC1. eauto. inversion H.
 Qed.
 
-(* Induction principle: preserves a predicate on C, st, e *)
-Lemma EreachE_ind_mut : 
-  forall (Pe : forall (C : dy_ctx) (st : state) (e : expr_tm), Prop)
-         (Pm : forall (C : dy_ctx) (st : state) (m : mod_tm), Prop),
-    (forall C st e, (Pe C st e) -> 
-      (match st with
-      | ST mem _ =>
-          forall addr,
-          match mem addr with
-            | None => True
-            | Some (Val v pf C') => Pe C' st v
-          end
-      end)) ->
-    (forall C st e1 e2,
-            Pe C st (e_app e1 e2) -> Pe C st e1) ->
-    (forall C st e1 e2 C_lam st_lam lam,
-            Pe C st (e_app e1 e2) -> 
-            Pe C_lam st_lam lam -> Pe C st_lam e2) ->
-    (forall C st e1 e2 C_lam st_lam x e
-            C_arg mem t arg pf,
-            Pe C st (e_app e1 e2) ->
-            Pe C_lam st_lam (e_lam x e) ->
-            Pe C_arg (ST mem t) arg ->
-            Pe (C_lam[|dy_c_lam x t  ([||])|])
-              (ST (t :: (dy_level C_lam) !-> (Val arg pf C_arg) ; mem) (update_t t)) e) ->
-    (forall C st m e, Pe C st (e_link m e) -> Pm C st m) ->
-    (forall C st m e C_m st_m,
-            Pe C st (e_link m e) -> (MevalR C st m C_m st_m) ->
-            Pm C_m st_m m_empty -> Pe C_m st_m e) ->
-    (forall C st M C_M (ACCESS : Some C_M = ctx_M C M),
-            Pm C st (m_var M) -> Pm C_M st m_empty) ->
-    (forall C st x e m,
-            Pm C st (m_lete x e m) -> Pe C st e) ->
-    (forall C st x e m C_x mem t v pf,
-            Pm C st (m_lete x e m) ->
-            Pe C_x (ST mem t) v ->
-            Pm (C[|dy_c_lete x t  ([||])|])
-              (ST (t :: (dy_level C) !-> (Val v pf C_x) ; mem) (update_t t)) m) ->
-    (forall C st M m1 m2,
-            Pm C st (m_letm M m1 m2) -> Pm C st m1) ->
-    (forall C st M m1 m2 C_M st_M,
-            Pm C st (m_letm M m1 m2) ->
-            (MevalR C st m1 C_M st_M) ->
-            Pm C_M st_M m_empty ->
-            Pm (C[|dy_c_letm M C_M  ([||])|]) st_M m2) ->
-    (forall C st e C' st' e'
-            (INIT : Pe C st e)
-            (REACH : <e| C st e ~> C' st' e' |e>),
-            Pe C' st' e').
-Proof. 
-(* intros just before our goal, then fix 8, on REACH, 
-   with mutual induction on EreachM, MreachE, MreachM *)
-  intros Pe Pm MEM APPl APPr APPb LINKm LINKe MVAR LETex LETem LETm1 LETm2.
-  fix IHere 8 with 
-    (IHerm C st e C' st' m'
-          (INIT : Pe C st e)
-          (REACH : <e| C st e ~> C' st' m' |m>)
-          { struct REACH }
-          : Pm C' st' m')
-    (IHmre C st m C' st' e'
-          (INIT : Pm C st m)
-          (REACH : <m| C st m ~> C' st' e' |e>)
-          { struct REACH }
-          : Pe C' st' e')
-    (IHmrm C st m C' st' m'
-          (INIT : Pm C st m)
-          (REACH : <m| C st m ~> C' st' m' |m>)
-          { struct REACH }
-          : Pm C' st' m').
-  - intros. destruct REACH.
-    + exact INIT.
-    + specialize (MEM C st (e_var x) INIT).
-      destruct st. specialize (MEM (addr_x C x)).
-      inversion STATE; subst. rewrite <- ACCESS in MEM.
-      exact MEM.
-    + apply (IHere C st e1 C' st' e'). eapply APPl.
-      exact INIT. exact REACH.
-    + apply (IHere C st_lam e2 C' st' e').
-      apply APPr with (st := st) (e1 := e1) (C_lam := C_lam) (lam := v).
-      exact INIT. apply (IHere C st e1 C_lam st_lam v).
-      eapply APPl. exact INIT. exact REACH1. exact REACH2.
-    + assert (LAM : Pe C_lam st_lam (e_lam x e)).
-      apply (IHere C st e1 C_lam st_lam (e_lam x e)).
-      eapply APPl. exact INIT. exact REACH1.
-      apply (IHere (C_lam [|dy_c_lam x t ([||])|])
-            (ST (t :: (dy_level C_lam) !-> Val arg pf C_arg; mem)
-            (update_t t)) e C' st' e').
-      apply APPb with (C := C) (st := st) (e1 := e1) (e2 := e2) (st_lam := st_lam).
-      exact INIT. exact LAM. 
-      apply (IHere C st_lam e2 C_arg (ST mem t) arg).
-      apply (APPr C st e1 e2 C_lam st_lam (e_lam x e)).
-      exact INIT. exact LAM. exact REACH2. exact REACH3.
-    + apply (IHmre C st m C' st' e'). apply LINKm with (e := e). exact INIT. exact REACHm.
-    + apply (IHere C_m st_m e C' st' e'). apply LINKe with (C := C) (st := st) (m := m).
-      exact INIT. exact MOD.
-      apply (IHmrm C st m C_m st_m m_empty).
-      eapply LINKm. exact INIT. exact MODr. exact REACH.
-  - intros. destruct REACH.
-    + apply (IHerm C st e1 C' st' m'). eapply APPl.
-      exact INIT. exact REACH.
-    + apply (IHerm C st_lam e2 C' st' m').
-      eapply APPr with (C_lam := C_lam) (lam := v). exact INIT.
-      apply (IHere C st e1 C_lam st_lam v).
-      eapply APPl. exact INIT. exact FNr. exact REACH.
-    + assert (LAM : Pe C_lam st_lam (e_lam x e)).
-      apply (IHere C st e1 C_lam st_lam (e_lam x e)).
-      eapply APPl. exact INIT. exact FNr.
-      apply (IHerm (C_lam [|dy_c_lam x t ([||])|])
-            (ST (t :: (dy_level C_lam) !-> Val arg pf C_arg; mem)
-            (update_t t)) e C' st' m').
-      eapply APPb with (st_lam := st_lam). exact INIT. exact LAM.
-      apply (IHere C st_lam e2 C_arg (ST mem t) arg).
-      apply (APPr C st e1 e2 C_lam st_lam (e_lam x e)).
-      exact INIT. exact LAM. exact ARGr. exact REACH.
-    + apply (IHmrm C st m C' st' m').
-      eapply LINKm. exact INIT. exact REACHm.
-    + apply (IHerm C_m st_m e C' st' m').
-      eapply LINKe. exact INIT. exact MOD.
-      apply (IHmrm C st m C_m st_m m_empty).
-      eapply LINKm. exact INIT. exact MODr. exact REACH.
-  - intros. destruct REACH.
-    + apply (IHere C st e C' st' e').
-      eapply LETex. exact INIT. exact REACHe.
-    + apply (IHmre (C [|dy_c_lete x t ([||])|])
-        (ST (t :: (dy_level C) !-> Val v pf C_x; mem) (update_t t)) m
-        C' st' e').
-      eapply LETem. exact INIT.
-      apply (IHere C st e C_x (ST mem t) v).
-      eapply LETex. exact INIT. exact EVALxr. exact REACH.
-    + apply (IHmre C st m1 C' st' e').
-      eapply LETm1. exact INIT. exact REACH.
-    + apply (IHmre (C [|dy_c_letm M C_M ([||])|]) st_M m2 C' st' e').
-      eapply LETm2. exact INIT. exact EVALM.
-      apply (IHmrm C st m1 C_M st_M m_empty).
-      eapply LETm1. exact INIT. exact EVALM0. exact REACH.
-  - intros. destruct REACH.
-    + exact INIT.
-    + specialize (MVAR C st M C_M ACCESS).
-      apply MVAR. exact INIT.
-    + apply (IHerm C st e C' st' m').
-      eapply LETex. exact INIT. exact REACHe.
-    + apply (IHmrm (C [|dy_c_lete x t ([||])|])
-        (ST (t :: (dy_level C) !-> Val v pf C_x; mem) (update_t t)) m
-        C' st' m').
-      eapply LETem. exact INIT.
-      apply (IHere C st e C_x (ST mem t) v).
-      eapply LETex. exact INIT. exact EVALxr. exact REACH.
-    + apply (IHmrm C st m1 C' st' m').
-      eapply LETm1. exact INIT. exact REACH.
-    + apply (IHmrm (C [|dy_c_letm M C_M ([||])|]) st_M m2 C' st' m').
-      eapply LETm2. exact INIT. exact EVALM.
-      apply (IHmrm C st m1 C_M st_M m_empty).
-      eapply LETm1. exact INIT. exact REACH1. exact REACH2.
-Qed.
-
-Lemma value_reach_only_itself_e :
+Lemma value_reach_only_itself :
   forall C st v (pf : value v)
          C' st' e'
-         (REACH : <e| C st v ~> C' st' e' |e>),
+         (REACH : <| C st v ~> C' st' e' |>),
          C = C' /\ st = st' /\ v = e'.
 Proof.
-  intros; repeat split; inversion pf; inversion REACH; subst; eauto using EreachE;
+  intros; repeat split; inversion pf; inversion REACH; subst; eauto using ReachR;
   try inversion H0.
-Qed.
-
-Lemma value_reach_only_itself_m :
-  forall C st v (pf : value v)
-         C' st' m'
-         (REACH : <e| C st v ~> C' st' m' |m>),
-         False.
-Proof.
-  intros; repeat split; inversion pf; inversion REACH; subst; eauto using EreachM;
-  try inversion H0.
-Qed.
-
-Lemma collect_ctx_expr_refl : forall e C, In C (collect_ctx_expr C e).
-Proof.
-  apply (expr_ind_mut
-    (fun e =>
-      forall C, In C (collect_ctx_expr C e))
-    (fun m =>
-      forall C, 
-        let (o, ctxs) := collect_ctx_mod C m in In C ctxs));
-  intros; simpl; eauto.
-  - apply in_app_iff. left. apply H.
-  - remember (collect_ctx_mod C m) as ol. destruct ol as [o l].
-    specialize (H C). rewrite <- Heqol in H.
-    destruct o; eauto. apply in_app_iff. left. eauto.
-  - destruct (st_ctx_M C M); simpl; left; eauto.
-  - destruct (collect_ctx_mod (C [[|st_c_lete x ([[||]])|]]) m).
-    apply in_app_iff. left. apply H.
-  - remember (collect_ctx_mod C m1) as ol.
-    destruct ol as [o l]. specialize (H C). rewrite <- Heqol in H.
-    destruct o; eauto.
-    + destruct (collect_ctx_mod (C [[|st_c_letm M s ([[||]])|]]) m2).
-      apply in_app_iff. left. eauto.
 Qed.
 
 Lemma Meval_then_collect :
-  forall C st m C_m st_m
-         (EVAL : MevalR C st m C_m st_m),
-        match collect_ctx_mod (dy_to_st C) m with
+  forall C st m v st_m
+         (EVAL : EvalR C st m v st_m)
+         C_m (MVAL : v = MVal C_m),
+        match collect_ctx (dy_to_st C) m with
         | (Some C_m', _) => C_m' = dy_to_st C_m
         | (None, _) => False
         end.
 Proof.
-  intros. induction EVAL; simpl; eauto.
-  - pose proof mod_is_static_some as H.
-    specialize (H C M). destruct H as [A B].
-    specialize (A C_M). symmetry in ACCESS.
-    specialize (A ACCESS). rewrite A. eauto.
-  - rewrite dy_to_st_plugin in IHEVAL.
-    simpl in IHEVAL.
-    remember (collect_ctx_mod (dy_to_st C [[|st_c_lete x ([[||]])|]]) m) as ol.
-    destruct ol. exact IHEVAL.
+  intros. revert C_m MVAL.
+  induction EVAL; intros; simpl; try inversion MVAL; subst; eauto.
+  - pose proof (mod_is_static_some C M) as H.
+    destruct H as [A B]. specialize (A C_m).
+    symmetry in ACCESS. specialize (A ACCESS).
+    rewrite A. eauto.
+  - rewrite dy_to_st_plugin in IHEVAL2.
+    simpl in IHEVAL2.
+    remember (collect_ctx (dy_to_st C [[|st_c_lete x ([[||]])|]]) m) as ol.
+    destruct ol. apply IHEVAL2; eauto.
   - rewrite dy_to_st_plugin in IHEVAL2. simpl in IHEVAL2.
-    destruct (collect_ctx_mod (dy_to_st C) m1). destruct o; try apply IHEVAL1.
+    specialize (IHEVAL1 C' eq_refl). specialize (IHEVAL2 C_m eq_refl).
+    destruct (collect_ctx (dy_to_st C) m'). destruct o; try apply IHEVAL1.
     rewrite <- IHEVAL1 in IHEVAL2.
-    destruct (collect_ctx_mod (dy_to_st C [[|st_c_letm M s ([[||]])|]]) m2).
-    exact IHEVAL2.
+    destruct (collect_ctx (dy_to_st C [[|st_c_letm M s ([[||]])|]]) m'').
+    apply IHEVAL2.
 Qed.
 
 Definition ctx_bound_st ub st:=
@@ -1095,122 +699,230 @@ Definition ctx_bound_st ub st:=
   | ST mem t =>
     forall addr,
       match mem addr with
-      | Some (Val v _ C_v) =>
-        forall sC (IN : In sC (collect_ctx_expr (dy_to_st C_v) v)),
+      | Some (Closure x e C_v) =>
+        let (o, ctxs) := collect_ctx (dy_to_st C_v) (e_lam x e) in
+        forall sC (IN : In sC ctxs),
                In sC ub
       | None => True
       end
   end.
 
-Definition ctx_bound_expr ub C st e :=
+Definition ctx_bound_tm ub C st e :=
   ctx_bound_st ub st /\
-  forall sC (IN : In sC (collect_ctx_expr (dy_to_st C) e)),
-         In sC ub.
-
-Definition ctx_bound_mod ub C st m :=
-  ctx_bound_st ub st /\
-  let (o, ctxs) := collect_ctx_mod (dy_to_st C) m in
+  let (o, ctxs) := collect_ctx (dy_to_st C) e in
   forall sC (IN : In sC ctxs),
          In sC ub.
 
-Lemma ere_ctx_bound :
+Lemma eval_ctx_bound :
+  forall ub
+         C st e
+         v st'
+         (INIT : ctx_bound_tm ub C st e)
+         (EVAL : EvalR C st e v st'),
+    match v with
+    | EVal (Closure x e' C_lam) =>
+      ctx_bound_tm ub C_lam st' (e_lam x e')
+    | MVal C_m =>
+      ctx_bound_tm ub C_m st' m_empty
+    (* | _ => ctx_bound_st ub st' *)
+    end.
+Proof.
+  intros. 
+  induction EVAL; try destruct v as [x' e' C_lam'];
+  destruct INIT as [A B].
+  - rewrite <- STATE in *. split; eauto.
+    specialize (A (addr_x C x)). rewrite <- ACCESS in A. eauto.
+  - destruct st. split; eauto.
+  - apply IHEVAL3. clear IHEVAL3.
+    simpl in B. 
+    assert (forall sC : st_ctx, In sC (snd (collect_ctx (dy_to_st C) e1)) -> In sC ub).
+    { intros. specialize (B sC). apply B. rewrite in_app_iff.
+      left. eauto. }
+    assert (ctx_bound_tm ub C st e1). 
+    { split; eauto. destruct (collect_ctx (dy_to_st C) e1); eauto. }
+    specialize (IHEVAL1 H0). clear H H0.
+    destruct IHEVAL1 as [A' B'].
+    assert (forall sC : st_ctx, In sC (snd (collect_ctx (dy_to_st C) e2)) -> In sC ub).
+    { intros. specialize (B sC). apply B. rewrite in_app_iff.
+      right. eauto. }
+    assert (ctx_bound_tm ub C st_lam e2).
+    { split; eauto. destruct (collect_ctx (dy_to_st C) e2); eauto. }
+    specialize (IHEVAL2 H0). clear H H0.
+    simpl in B'. split; 
+    try (rewrite dy_to_st_plugin; simpl;
+         (destruct (collect_ctx (dy_to_st C_lam [[|st_c_lam x ([[||]])|]]) e));
+         simpl in B'; intros; apply B'; eauto).
+    simpl. intros. unfold update_m. 
+    destruct arg as [x'' e'' C_lam''].
+    destruct IHEVAL2 as [A'' B''].
+    destruct (eq_p addr (t :: dy_level C_lam)); eauto.
+    simpl in A''. apply A''.
+  - apply IHEVAL2. clear IHEVAL2.
+    simpl in B.
+    assert (forall sC : st_ctx, In sC (snd (collect_ctx (dy_to_st C) m)) -> In sC ub).
+    { intros. destruct (collect_ctx (dy_to_st C) m). 
+      destruct o; specialize (B sC); apply B. 
+      rewrite in_app_iff. left; eauto. eauto. }
+    assert (ctx_bound_tm ub C st m). 
+    { split; eauto. destruct (collect_ctx (dy_to_st C) m); eauto. }
+    specialize (IHEVAL1 H0). clear H H0.
+    destruct IHEVAL1 as [A' B'].
+    split; eauto. eapply Meval_then_collect in EVAL1; eauto.
+    destruct (collect_ctx (dy_to_st C) m). 
+    destruct o; try (inversion EVAL1; fail).
+    rewrite <- EVAL1. destruct (collect_ctx s e).
+    simpl in B. intros. apply B. rewrite in_app_iff. right; eauto.
+  - split; eauto.
+  - split; eauto. simpl in *.
+    pose proof (mod_is_static_some C M) as H.
+    destruct H as [A' B']. symmetry in ACCESS. 
+    specialize (A' C_M ACCESS). rewrite A' in B.
+    intros. destruct IN as [IN | contra]; try inversion contra.
+    apply B. simpl. right. left. eauto.
+  - apply IHEVAL2. clear IHEVAL2.
+    simpl in B. 
+    assert (forall sC : st_ctx, In sC (snd (collect_ctx (dy_to_st C) e)) -> In sC ub).
+    { intros. destruct (collect_ctx (dy_to_st C [[|st_c_lete x ([[||]])|]]) m).
+      specialize (B sC). apply B. rewrite in_app_iff.
+      left. eauto. }
+    assert (ctx_bound_tm ub C st e). 
+    { split; eauto. destruct (collect_ctx (dy_to_st C) e); eauto. }
+    specialize (IHEVAL1 H0). clear H H0.
+    destruct IHEVAL1 as [A' B'].
+    split;
+    try (rewrite dy_to_st_plugin; simpl;
+         (destruct (collect_ctx (dy_to_st C [[|st_c_lete x ([[||]])|]]) m));
+         simpl in B; intros; apply B; rewrite in_app_iff; right; 
+         eauto).
+    simpl. intros. unfold update_m. 
+    destruct (eq_p addr (t :: dy_level C)); eauto.
+    simpl in A'. apply A'.
+  - apply IHEVAL2. clear IHEVAL2.
+    simpl in B. 
+    assert (forall sC : st_ctx, In sC (snd (collect_ctx (dy_to_st C) m')) -> In sC ub).
+    { intros. destruct (collect_ctx (dy_to_st C) m'). 
+      destruct o; eauto. destruct (collect_ctx (dy_to_st C [[|st_c_letm M s ([[||]])|]]) m'').
+      specialize (B sC). apply B. rewrite in_app_iff.
+      left. eauto. }
+    assert (ctx_bound_tm ub C st m'). 
+    { split; eauto. destruct (collect_ctx (dy_to_st C) m'); eauto. }
+    specialize (IHEVAL1 H0). clear H H0.
+    destruct IHEVAL1 as [A' B'].
+    split; eauto.
+    rewrite dy_to_st_plugin; simpl.
+    eapply Meval_then_collect in EVAL1; eauto.
+    destruct (collect_ctx (dy_to_st C) m'). 
+    destruct o; try inversion EVAL1. clear H. rewrite <- EVAL1.
+    destruct (collect_ctx (dy_to_st C [[|st_c_letm M s ([[||]])|]]) m'').
+    intros. apply B. rewrite in_app_iff. right; eauto.
+Qed.
+
+Lemma reach_ctx_bound :
   forall ub
          C st e
          C' st' e'
-         (INIT : ctx_bound_expr ub C st e)
-         (REACH : <e| C st e ~> C' st' e' |e>),
-    ctx_bound_expr ub C' st' e'.
+         (INIT : ctx_bound_tm ub C st e)
+         (REACH : <| C st e ~> C' st' e' |>),
+    ctx_bound_tm ub C' st' e'.
 Proof.
-  intros ub.
-  apply (EreachE_ind_mut (ctx_bound_expr ub) (ctx_bound_mod ub)).
-  - intros. unfold ctx_bound_expr in *. destruct H as [mem expr].
-    destruct st. intros. remember (mem0 addr) as v.
-    destruct v; eauto. destruct e0.
-    split; eauto.
-    unfold ctx_bound_st in *. specialize (mem addr).
-    rewrite <- Heqv in mem. eauto.
-  - intros. unfold ctx_bound_expr in *. destruct H as [mem expr].
-    split; eauto. intros. specialize (expr sC).
-    assert (In sC (collect_ctx_expr (dy_to_st C) (e_app e1 e2))).
-    simpl. apply in_app_iff. left. eauto. eauto.
-  - intros. unfold ctx_bound_expr in *. destruct H as [memi expri].
-    destruct H0 as [memlam exprlam]. split; eauto.
-    intros. specialize (expri sC). specialize (exprlam sC).
-    assert (In sC (collect_ctx_expr (dy_to_st C) (e_app e1 e2))).
-    simpl. apply in_app_iff. right. eauto. eauto.
-  - intros. unfold ctx_bound_expr in *. destruct H as [memi expri].
-    destruct H0 as [memlam exprlam]. destruct H1 as [memarg exprarg].
-    split. 
-    + unfold ctx_bound_st. unfold update_m. intro addr.
-      destruct (eq_p addr (t :: (dy_level C_lam))). exact exprarg.
-      apply memarg. 
-    + rewrite dy_to_st_plugin. simpl. remember (dy_to_st C_lam) as st_C.
-      simpl in exprlam. eauto.
-  - intros C st m e [mem expr]. split. exact mem.
-    simpl in expr. remember (collect_ctx_mod (dy_to_st C) m) as ol.
-    destruct ol. destruct o; intros; specialize (expr sC).
-    + assert (In sC (l ++ collect_ctx_expr s e)) as HINT.
-      apply in_app_iff. left; eauto. eauto.
-    + apply expr. eauto.
-  - intros C st m e C_m st_m [mem expr] meval [memm exprm]. split. exact memm.
-    apply Meval_then_collect in meval.
-    simpl in expr. simpl in exprm. remember (collect_ctx_mod (dy_to_st C) m) as ol.
-    destruct ol; destruct o; intros; specialize (expr sC). 
-    + rewrite <- meval in *. 
-      assert (In sC (l ++ collect_ctx_expr s e)) as HINT.
-      apply in_app_iff. right. eauto. eauto.
-    + inversion meval.
-  - intros C st M C_M ACCESS [mem expr].
-    split. exact mem. simpl in expr.
-    pose proof mod_is_static_some as MOD.
-    specialize (MOD C M). destruct MOD as [MODl MODr].
-    symmetry in ACCESS. specialize (MODl C_M ACCESS).
-    rewrite MODl in expr. simpl. intros; inversion IN; try inversion H.
-    specialize (expr (dy_to_st C_M)).
-    assert (In (dy_to_st C_M) [dy_to_st C; dy_to_st C_M]) as HINT.
-    simpl; right; eauto. eauto.
-  - intros C st x e m [mem expr].
-    split. exact mem. simpl in expr.
-    destruct (collect_ctx_mod (st_c_plugin (dy_to_st C) (st_c_lete x st_c_hole)) m).
-    intros. specialize (expr sC).
-    assert (In sC (collect_ctx_expr (dy_to_st C) e ++ l)) as HINT.
-    apply in_app_iff. left. eauto. eauto.
-  - intros C st x e m C_x mem t v pf 
-    [memi expri] [memm exprm]. split.
-    + unfold ctx_bound_st. unfold update_m. intro addr.
-      destruct (eq_p addr (t :: (dy_level C))). exact exprm.
-      apply memm.
-    + simpl in expri. rewrite dy_to_st_plugin. simpl.
-      destruct (collect_ctx_mod (st_c_plugin (dy_to_st C) (st_c_lete x st_c_hole)) m).
-      intros. specialize (expri sC).
-      assert (In sC (collect_ctx_expr (dy_to_st C) e ++ l)) as HINT.
-      apply in_app_iff. right. eauto. eauto.
-  - intros C st M m1 m2 [mem expr]. split. exact mem. simpl in expr.
-    destruct (collect_ctx_mod (dy_to_st C) m1). destruct o; eauto.
-    destruct (collect_ctx_mod (st_c_plugin (dy_to_st C) (st_c_letm M s st_c_hole)) m2). destruct o;
-    intros; specialize (expr sC); 
-    assert (In sC (l ++ l0)) as HINT; try apply in_app_iff; try left; eauto.
-  - intros C st M m1 m2 C_M st_M [memi expri] meval [memm exprm].
-    apply Meval_then_collect in meval. simpl in expri. simpl in exprm.
-    remember (collect_ctx_mod (dy_to_st C) m1) as ol1. 
-    destruct ol1. destruct o; unfold ctx_bound_mod in *;
-    rewrite dy_to_st_plugin in *; simpl; split; try inversion meval; 
-    try rewrite <- meval; eauto.
-    destruct (collect_ctx_mod (dy_to_st C [[|st_c_letm M s ([[||]])|]]) m2).
-    intros. assert (In sC (l ++ l0)) as HINT. apply in_app_iff. right. eauto. eauto.
+  intros. induction REACH; eauto; 
+          apply IHREACH; destruct INIT as [A B].
+  - simpl in B. split; eauto.
+    destruct (collect_ctx (dy_to_st C) e1).
+    intros; apply B. simpl in *. rewrite in_app_iff. left; eauto.
+  - apply eval_ctx_bound with (ub := ub) in FN.
+    destruct FN as [A' B'].
+    split; eauto. simpl in B.
+    destruct (collect_ctx (dy_to_st C) e2).
+    intros; apply B. simpl in *. rewrite in_app_iff. right; eauto.
+    split; eauto. simpl in B.
+    destruct (collect_ctx (dy_to_st C) e1).
+    intros; apply B. simpl in *. rewrite in_app_iff. left; eauto.
+  - apply eval_ctx_bound with (ub := ub) in FN.
+    apply eval_ctx_bound with (ub := ub) in ARG. destruct arg as [x'' e'' C''].
+    destruct FN as [A' B']. destruct ARG as [A'' B''].
+    split. simpl. intros. unfold update_m.
+    destruct (eq_p addr (t :: dy_level C_lam)).
+    simpl in B''. apply B''.
+    simpl in A''. apply A''.
+    rewrite dy_to_st_plugin. simpl. simpl in B'.
+    destruct (collect_ctx (dy_to_st C_lam [[|st_c_lam x ([[||]])|]]) e).
+    simpl in B'. intros; apply B'. right; eauto.
+    destruct FN as [A' B'].
+    split; eauto. simpl in B.
+    destruct (collect_ctx (dy_to_st C) e2).
+    intros; apply B. simpl in *. rewrite in_app_iff. right; eauto.
+    split; eauto. simpl in B.
+    destruct (collect_ctx (dy_to_st C) e1).
+    intros; apply B. simpl in *. rewrite in_app_iff. left; eauto.
+  - split; eauto. simpl in B.
+    destruct (collect_ctx (dy_to_st C) m). 
+    intros. destruct o; apply B; eauto.
+    rewrite in_app_iff. left; eauto.
+  - eapply Meval_then_collect in MOD as MOD'; eauto.
+    apply eval_ctx_bound with (ub := ub) in MOD.
+    destruct MOD as [A' B'].
+    split; eauto. simpl in B.
+    destruct (collect_ctx (dy_to_st C) m).
+    destruct o; inversion MOD'. clear H. rewrite <- MOD'.
+    destruct (collect_ctx s e). 
+    intros; apply B; simpl; rewrite in_app_iff; right; eauto.
+    split; eauto. simpl in B.
+    destruct (collect_ctx (dy_to_st C) m). 
+    intros. destruct o; apply B; eauto.
+    rewrite in_app_iff. left; eauto.
+  - split; eauto. simpl in B.
+    destruct (collect_ctx (dy_to_st C) e).
+    destruct (collect_ctx (dy_to_st C [[|st_c_lete x ([[||]])|]]) m). 
+    intros; apply B; simpl; rewrite in_app_iff; left; eauto.
+  - apply eval_ctx_bound with (ub := ub) in EVALx. destruct v as [x'' e'' C_lam''].
+    destruct EVALx as [A' B'].
+    split.
+    simpl; intros. unfold update_m.
+    destruct (eq_p addr (t :: dy_level C)).
+    simpl in B'; eauto. simpl in A'; apply A'.
+    simpl in B. rewrite dy_to_st_plugin. simpl.
+    destruct (collect_ctx (dy_to_st C [[|st_c_lete x ([[||]])|]]) m).
+    intros; apply B. rewrite in_app_iff; right; eauto.
+    (* copy of the goal before *)
+    split; eauto. simpl in B.
+    destruct (collect_ctx (dy_to_st C) e).
+    destruct (collect_ctx (dy_to_st C [[|st_c_lete x ([[||]])|]]) m). 
+    intros; apply B; simpl; rewrite in_app_iff; left; eauto.
+  - split; eauto. simpl in B.
+    destruct (collect_ctx (dy_to_st C) m1). destruct o; eauto.
+    destruct (collect_ctx (dy_to_st C [[|st_c_letm M s ([[||]])|]]) m2). 
+    intros; apply B; simpl; rewrite in_app_iff; left; eauto.
+  - eapply Meval_then_collect in EVALM as EVALM'; eauto.
+    apply eval_ctx_bound with (ub := ub) in EVALM.
+    destruct EVALM as [A' B'].
+    split; eauto. simpl in B.
+    destruct (collect_ctx (dy_to_st C) m1). destruct o; inversion EVALM'.
+    clear H. rewrite dy_to_st_plugin; simpl. rewrite <- EVALM'.
+    destruct (collect_ctx (dy_to_st C [[|st_c_letm M s ([[||]])|]]) m2).
+    intros; apply B; rewrite in_app_iff; right; eauto.
+    (* copy of the goal before *)
+    split; eauto. simpl in B.
+    destruct (collect_ctx (dy_to_st C) m1). destruct o; eauto.
+    destruct (collect_ctx (dy_to_st C [[|st_c_letm M s ([[||]])|]]) m2). 
+    intros; apply B; simpl; rewrite in_app_iff; left; eauto.
 Qed.
 
 Theorem expr_ctx_bound :
   forall e C' st' e'
-         (REACH : <e|  ([||]) (ST empty_mem 0) e ~> C' st' e' |e>),
-         In (dy_to_st C') (collect_ctx_expr ([[||]]) e).
+         (REACH : <| ([||]) (ST empty_mem 0) e ~> C' st' e' |>),
+         In (dy_to_st C') (snd (collect_ctx ([[||]]) e)).
 Proof.
   intros.
-  pose proof (ere_ctx_bound (collect_ctx_expr st_c_hole e)  ([||]) (ST empty_mem 0) e C' st' e') as H.
-  assert (ctx_bound_expr (collect_ctx_expr ([[||]]) e)  ([||])
-          (ST empty_mem 0) e) as FINAL.
-  - unfold ctx_bound_expr; split; simpl; eauto.
+  pose proof (reach_ctx_bound (snd (collect_ctx st_c_hole e)) ([||]) (ST empty_mem 0) e C' st' e') as H.
+  assert (ctx_bound_tm (snd (collect_ctx ([[||]]) e)) 
+                       ([||]) (ST empty_mem 0) e) as FINAL.
+  - split; simpl; eauto. destruct (collect_ctx ([[||]]) e); eauto.
   - apply H in FINAL; try apply REACH. 
     destruct FINAL as [MEM KILLER].
-    apply KILLER. apply collect_ctx_expr_refl.
+    remember (collect_ctx (dy_to_st C') e') as ol.
+    destruct ol. apply KILLER. 
+    assert (l = (snd (collect_ctx (dy_to_st C') e'))) as RR.
+    rewrite <- Heqol; eauto.
+    rewrite RR. apply collect_ctx_refl.
 Qed.
