doc/coq/Sound.v
@@ -23,8 +23,8 @@ Definition time_bound C st :=
       mem p = None) /\
     (forall p (BOUND : p_bound p t),
       match mem p with
-      | None => True
-      | Some (Val _ _ C') => dy_ctx_bound C' t
+      | Some (Closure _ _ C') => dy_ctx_bound C' t
+      | _ => True
       end)
   end.
 
@@ -69,9 +69,9 @@ Definition sound α C st abs_C abs_st :=
       forall p (BOUND : p_bound p t),
         match mem p with
         | None => True
-        | Some (Val v pf Cv) =>
+        | Some (Closure x e Cv) =>
           let l := abs_mem (map α p) in
-          In (Abstract.Val v pf (trans_ctx α Cv)) l
+          In (Abstract.Closure x e (trans_ctx α Cv)) l
         end
     end
   end.
@@ -93,42 +93,57 @@ Proof.
     rewrite map_app. eauto.
 Qed.
 
-Lemma time_increase_e :
-  forall C st e e' st'
-         (EVAL : EevalR C st e e' st'),
-    match st with
-    | ST _ t =>
-      match st' with
-      | ST _ t' => t <= t'
-      end
-    end.
+Lemma trans_ctx_ctx_M :
+  forall C α abs_C M C_M
+        (ACCESS : ctx_M C M = Some C_M)
+        (TRANS : trans_ctx α C = abs_C),
+    Abstract.ctx_M abs_C M = Some (trans_ctx α C_M).
 Proof.
-  apply (EevalR_ind_mut
-    (fun C st e e' st'
-         (EVAL : EevalR C st e e' st') =>
-      match st with
-      | ST _ t =>
-        match st' with
-        | ST _ t' => t <= t'
-        end
-      end)
-    (fun C st m C' st'
-         (EVAL : MevalR C st m C' st') =>
-      match st with
-      | ST _ t =>
-        match st' with
-        | ST _ t' => t <= t'
-        end
-      end)); 
-      intros; 
-      destruct st; try destruct st'; try destruct st_v; try destruct st_m; 
-      try destruct st_m1; try destruct st_m2; try destruct st_lam;
-      unfold update_t in *; simpl; try nia.
+  assert (forall C α M,
+    match Abstract.ctx_M (trans_ctx α C) M with
+    | Some _ => 
+      match ctx_M C M with
+      | Some _ => True
+      | None => False
+      end
+    | None =>
+      match ctx_M C M with
+      | Some _ => False
+      | None => True
+      end
+    end).
+  {
+    induction C; intros; simpl; eauto; try apply IHC.
+    destruct (eq_mid M0 M); 
+    remember (Abstract.ctx_M (trans_ctx α C2) M0) as ctx';
+    destruct ctx';
+    specialize (IHC2 α M0);
+    rewrite <- Heqctx' in IHC2;
+    destruct (ctx_M C2 M0);
+    try inversion IHC2; eauto.
+  }
+  induction C; intros; simpl in *; eauto.
+  - inversion ACCESS.
+  - rewrite <- TRANS. simpl. apply IHC; eauto.
+  - rewrite <- TRANS. simpl. apply IHC; eauto. 
+  - rewrite <- TRANS. simpl.
+    remember (Abstract.ctx_M (trans_ctx α C2) M0) as ctx1.
+    destruct ctx1; try (inversion ACCESS; fail).
+    + specialize (H C2 α M0).
+      rewrite <- Heqctx1 in H.
+      remember (ctx_M C2 M0) as ctx2; destruct ctx2;
+      inversion H; inversion ACCESS; subst.
+      rewrite Heqctx1. apply IHC2; eauto.
+    + specialize (H C2 α M0).
+      rewrite <- Heqctx1 in H.
+      remember (ctx_M C2 M0) as ctx2; destruct ctx2;
+      inversion H; destruct (eq_mid M0 M);
+      inversion ACCESS; subst; eauto.
 Qed.
 
-Lemma time_increase_m :
-  forall C st m C' st'
-         (EVAL : MevalR C st m C' st'),
+Lemma time_increase_e :
+  forall C st e e' st'
+         (EVAL : EvalR C st e e' st'),
     match st with
     | ST _ t =>
       match st' with
@@ -136,27 +151,12 @@ Lemma time_increase_m :
       end
     end.
 Proof.
-  apply (MevalR_ind_mut
-    (fun C st e e' st'
-         (EVAL : EevalR C st e e' st') =>
-      match st with
-      | ST _ t =>
-        match st' with
-        | ST _ t' => t <= t'
-        end
-      end)
-    (fun C st m C' st'
-         (EVAL : MevalR C st m C' st') =>
-      match st with
-      | ST _ t =>
-        match st' with
-        | ST _ t' => t <= t'
-        end
-      end)); 
-      intros; 
-      destruct st; try destruct st'; try destruct st_v; try destruct st_m; 
-      try destruct st_m1; try destruct st_m2; try destruct st_lam;
-      unfold update_t in *; simpl; try nia.
+  intros. 
+  induction EVAL;
+  intros; 
+  destruct st; try destruct st'; try destruct st''; try destruct st_v; 
+  try destruct st_m; try destruct st_lam;
+  unfold update_t in *; simpl; try nia.
 Qed.
 
 Lemma relax_ctx_bound :
@@ -239,82 +239,75 @@ Qed.
 
 Lemma time_bound_e :
   forall C st e e' st'
-         (EVAL : EevalR C st e e' st')
+         (EVAL : EvalR C st e e' st')
          (BOUND : time_bound C st),
     match e' with
-    | Val _ _ C' => time_bound C' st'
+    | EVal (Closure _ _ C') => time_bound C' st'
+    | MVal C' => time_bound C' st'
     end.
 Proof.
-  apply (EevalR_ind_mut
-    (fun C st e e' st'
-         (EVAL : EevalR C st e e' st') =>
-      forall (BOUND : time_bound C st),
-        match e' with
-        | Val _ _ C' => time_bound C' st'
-        end)
-    (fun C st m C' st'
-         (EVAL : MevalR C st m C' st') =>
-      forall (BOUND : time_bound C st), 
-        time_bound C' st')); intros; simpl; eauto.
+  intros. induction EVAL; intros; simpl; eauto.
   - destruct v. unfold time_bound in *.
     destruct st. destruct BOUND as [? [? RR]].
     specialize (RR (addr_x C x)) as RR'.
     assert (p_bound (addr_x C x) t0). apply time_bound_addr. eauto.
     apply RR' in H1. inversion STATE; subst. 
     rewrite <- ACCESS in H1. repeat split; eauto.
-  - specialize (H BOUND). 
+  - specialize (IHEVAL1 BOUND). 
     destruct v. destruct arg. 
     destruct st. destruct st_lam. destruct st_v.
-    apply time_increase_e in ARG as time_inc1.
-    apply time_increase_e in FN as time_inc2.
-    apply time_increase_e in BODY as time_inc3.
+    apply time_increase_e in EVAL1 as time_inc1.
+    apply time_increase_e in EVAL2 as time_inc2.
+    apply time_increase_e in EVAL3 as time_inc3.
     assert (time_bound C (ST mem1 t1)) as HINT.
     {
-      simpl in H. destruct H as [? [? ?]]. 
+      simpl in IHEVAL1. destruct IHEVAL1 as [? [? ?]]. 
       simpl; repeat split; eauto. 
       eapply relax_ctx_bound. 
       simpl in BOUND. destruct BOUND. exact d. eauto. 
     }
-    specialize (H0 HINT).
-    assert (p_bound (t :: dy_level C_lam) (update_t t)).
+    specialize (IHEVAL2 HINT).
+    assert (p_bound (t :: dy_level C_lam) (update_t C (ST mem t) x (Closure x1 e3 C1))).
     {
-      simpl in H. destruct H as [? [? ?]].
+      simpl in IHEVAL1. destruct IHEVAL1 as [? [? ?]].
       simpl. split; unfold update_t; eauto.
       apply relax_p_bound with (t1 := t1).
       apply time_bound_level. eauto. nia.
     }
-    apply H1; simpl. split.
+    apply IHEVAL3; simpl. split.
     rewrite plugin_ctx_bound. split.
-    simpl in H. destruct H as [? [? ?]].
-    eapply relax_ctx_bound. exact H. unfold update_t. nia.
-    simpl. split; eauto. simpl in H0. destruct H0 as [? [? ?]].
+    simpl in IHEVAL1. destruct IHEVAL1 as [? [? ?]].
+    eapply relax_ctx_bound. eauto. nia.
+    simpl. split; eauto.
     split; intros;
     unfold update_m; remember (eq_p p (t :: dy_level C_lam)) as b;
     destruct b; symmetry in Heqb; try rewrite eq_p_eq in Heqb.
-    + assert (p_bound p (update_t t)) as contra. { rewrite Heqb. eauto. }
+    + assert (p_bound p (S t)) as contra. { rewrite Heqb. eauto. }
       apply NBOUND in contra. inversion contra.
-    + apply H3.
-      unfold not. intros.
-      assert (p_bound p (update_t t)) as contra. 
-      { apply relax_p_bound with (t1 := t). eauto. unfold update_t; eauto. }
+    + simpl in IHEVAL2. destruct IHEVAL2 as [? [RR ?]].
+      apply RR. unfold not. intros. 
+      assert (p_bound p (S t)) as contra.
+      apply relax_p_bound with (t1 := t); eauto. 
       apply NBOUND in contra. inversion contra.
-    + apply relax_ctx_bound with (t1 := t). eauto. unfold update_t; eauto.
-    + specialize (H4 p). remember (mem p) as access eqn:ACCESS.
-      destruct access; eauto. destruct e0.
-      apply relax_ctx_bound with (t1 := t). apply H4.
+    + apply relax_ctx_bound with (t1 := t); eauto.
+      simpl in IHEVAL2. destruct IHEVAL2 as [? [? ?]]; eauto.
+    + destruct IHEVAL2 as [? [? RR]]. 
+      specialize (RR p). remember (mem p) as access eqn:ACCESS.
+      destruct access; eauto. destruct e4.
+      apply relax_ctx_bound with (t1 := t); eauto. apply RR.
       pose proof (p_bound_or_not p t) as CASES.
-      destruct CASES as [? | contra]; eauto. apply H3 in contra.
-      rewrite contra in ACCESS. inversion ACCESS. unfold update_t. eauto.
-  - apply H0. apply H. eauto.
+      destruct CASES as [? | contra]; eauto.
+      specialize (H1 p contra). rewrite H1 in ACCESS. inversion ACCESS.
+  - apply IHEVAL2. apply IHEVAL1. eauto.
   - destruct st. simpl in *. destruct BOUND as [? [? ?]].
     repeat split; eauto. eapply time_bound_ctx_M.
     symmetry. exact ACCESS. eauto.
-  - specialize (H BOUND).
-    destruct v_e. 
+  - specialize (IHEVAL1 BOUND).
+    destruct v. 
     destruct st. destruct st_m.
-    apply time_increase_e in EVALe as time_inc1.
-    apply time_increase_m in EVALm as time_inc2.
-    assert (p_bound (t :: dy_level C) (update_t t)).
+    apply time_increase_e in EVAL1 as time_inc1.
+    apply time_increase_e in EVAL2 as time_inc2.
+    assert (p_bound (t :: dy_level C) (update_t C (ST mem t) x (Closure x0 e0 C0))).
     {
       simpl in BOUND. destruct BOUND as [? [? ?]].
       simpl. split; unfold update_t; eauto.
@@ -322,150 +315,33 @@ Proof.
       apply time_bound_level. eauto. nia.
     }
     simpl in BOUND. destruct BOUND as [B1 [B2 B3]].
-    simpl in H. destruct H as [HH1 [HH2 HH3]].
-    apply H0. simpl; split.
+    simpl in IHEVAL1. destruct IHEVAL1 as [HH1 [HH2 HH3]].
+    apply IHEVAL2. simpl; split.
     rewrite plugin_ctx_bound; split.
-    apply relax_ctx_bound with (t1 := t0).
-    eauto. unfold update_t. nia. simpl; split; eauto.
+    apply relax_ctx_bound with (t1 := t0); eauto. simpl; split; eauto.
     split; intros;
     unfold update_m; remember (eq_p p (t :: dy_level C)) as b;
     destruct b; symmetry in Heqb; try rewrite eq_p_eq in Heqb.
-    + assert (p_bound p (update_t t)) as contra. { rewrite Heqb. eauto. }
+    + assert (p_bound p (S t)) as contra. { rewrite Heqb. eauto. }
       apply NBOUND in contra. inversion contra.
-    + apply HH2. unfold not. intros.
-      assert (p_bound p (update_t t)) as contra. 
-      { apply relax_p_bound with (t1 := t). eauto. unfold update_t; eauto. }
+    + apply HH2. unfold not. intros. 
+      assert (p_bound p (S t)) as contra.
+      apply relax_p_bound with (t1 := t); eauto. 
       apply NBOUND in contra. inversion contra.
-    + apply relax_ctx_bound with (t1 := t). eauto. unfold update_t; eauto.
+    + apply relax_ctx_bound with (t1 := t); eauto.
     + specialize (HH3 p). remember (mem p) as access eqn:ACCESS.
-      destruct access; eauto. destruct e0.
-      apply relax_ctx_bound with (t1 := t). apply HH3.
+      destruct access; eauto. destruct e1.
+      apply relax_ctx_bound with (t1 := t); eauto. apply HH3.
       pose proof (p_bound_or_not p t) as CASES.
-      destruct CASES as [? | contra]; eauto. apply HH2 in contra.
-      rewrite contra in ACCESS. inversion ACCESS. unfold update_t. eauto.
-  - specialize (H BOUND).
-    destruct st. destruct st_m1. destruct st_m2.
+      destruct CASES as [? | contra]; eauto.
+      specialize (HH2 p contra). rewrite HH2 in ACCESS. inversion ACCESS.
+  - specialize (IHEVAL1 BOUND).
+    destruct st. destruct st'. destruct st''.
     simpl in BOUND. destruct BOUND as [B1 [B2 B3]].
-    simpl in H. destruct H as [HH1 [HH2 HH3]].
-    apply time_increase_m in EVALm1 as time_inc1.
-    apply time_increase_m in EVALm2 as time_inc2.
-    apply H0. simpl. repeat split; eauto.
-    rewrite plugin_ctx_bound. split.
-    apply relax_ctx_bound with (t1 := t); eauto.
-    simpl; split; eauto.
-Qed.
-
-Lemma time_bound_m :
-  forall C st m C' st'
-         (EVAL : MevalR C st m C' st')
-         (BOUND : time_bound C st),
-    time_bound C' st'.
-Proof.
-  apply (MevalR_ind_mut
-    (fun C st e e' st'
-         (EVAL : EevalR C st e e' st') =>
-      forall (BOUND : time_bound C st),
-        match e' with
-        | Val _ _ C' => time_bound C' st'
-        end)
-    (fun C st m C' st'
-         (EVAL : MevalR C st m C' st') =>
-      forall (BOUND : time_bound C st), 
-        time_bound C' st')); intros; simpl; eauto.
-  - destruct v. unfold time_bound in *.
-    destruct st. destruct BOUND as [? [? RR]].
-    specialize (RR (addr_x C x)) as RR'.
-    assert (p_bound (addr_x C x) t0). apply time_bound_addr. eauto.
-    apply RR' in H1. inversion STATE; subst. 
-    rewrite <- ACCESS in H1. repeat split; eauto.
-  - specialize (H BOUND). 
-    destruct v. destruct arg. 
-    destruct st. destruct st_lam. destruct st_v.
-    apply time_increase_e in ARG as time_inc1.
-    apply time_increase_e in FN as time_inc2.
-    apply time_increase_e in BODY as time_inc3.
-    assert (time_bound C (ST mem1 t1)) as HINT.
-    {
-      simpl in H. destruct H as [? [? ?]]. 
-      simpl; repeat split; eauto. 
-      eapply relax_ctx_bound. 
-      simpl in BOUND. destruct BOUND. exact d. eauto. 
-    }
-    specialize (H0 HINT).
-    assert (p_bound (t :: dy_level C_lam) (update_t t)).
-    {
-      simpl in H. destruct H as [? [? ?]].
-      simpl. split; unfold update_t; eauto.
-      apply relax_p_bound with (t1 := t1).
-      apply time_bound_level. eauto. nia.
-    }
-    apply H1; simpl. split.
-    rewrite plugin_ctx_bound. split.
-    simpl in H. destruct H as [? [? ?]].
-    eapply relax_ctx_bound. exact H. unfold update_t. nia.
-    simpl. split; eauto. simpl in H0. destruct H0 as [? [? ?]].
-    split; intros;
-    unfold update_m; remember (eq_p p (t :: dy_level C_lam)) as b;
-    destruct b; symmetry in Heqb; try rewrite eq_p_eq in Heqb.
-    + assert (p_bound p (update_t t)) as contra. { rewrite Heqb. eauto. }
-      apply NBOUND in contra. inversion contra.
-    + apply H3.
-      unfold not. intros.
-      assert (p_bound p (update_t t)) as contra. 
-      { apply relax_p_bound with (t1 := t). eauto. unfold update_t; eauto. }
-      apply NBOUND in contra. inversion contra.
-    + apply relax_ctx_bound with (t1 := t). eauto. unfold update_t; eauto.
-    + specialize (H4 p). remember (mem p) as access eqn:ACCESS.
-      destruct access; eauto. destruct e0.
-      apply relax_ctx_bound with (t1 := t). apply H4.
-      pose proof (p_bound_or_not p t) as CASES.
-      destruct CASES as [? | contra]; eauto. apply H3 in contra.
-      rewrite contra in ACCESS. inversion ACCESS. unfold update_t. eauto.
-  - apply H0. apply H. eauto.
-  - destruct st. simpl in *. destruct BOUND as [? [? ?]].
-    repeat split; eauto. eapply time_bound_ctx_M.
-    symmetry. exact ACCESS. eauto.
-  - specialize (H BOUND).
-    destruct v_e. 
-    destruct st. destruct st_m.
-    apply time_increase_e in EVALe as time_inc1.
-    apply time_increase_m in EVALm as time_inc2.
-    assert (p_bound (t :: dy_level C) (update_t t)).
-    {
-      simpl in BOUND. destruct BOUND as [? [? ?]].
-      simpl. split; unfold update_t; eauto.
-      apply relax_p_bound with (t1 := t0).
-      apply time_bound_level. eauto. nia.
-    }
-    simpl in BOUND. destruct BOUND as [B1 [B2 B3]].
-    simpl in H. destruct H as [HH1 [HH2 HH3]].
-    apply H0. simpl; split.
-    rewrite plugin_ctx_bound; split.
-    apply relax_ctx_bound with (t1 := t0).
-    eauto. unfold update_t. nia. simpl; split; eauto.
-    split; intros;
-    unfold update_m; remember (eq_p p (t :: dy_level C)) as b;
-    destruct b; symmetry in Heqb; try rewrite eq_p_eq in Heqb.
-    + assert (p_bound p (update_t t)) as contra. { rewrite Heqb. eauto. }
-      apply NBOUND in contra. inversion contra.
-    + apply HH2. unfold not. intros.
-      assert (p_bound p (update_t t)) as contra. 
-      { apply relax_p_bound with (t1 := t). eauto. unfold update_t; eauto. }
-      apply NBOUND in contra. inversion contra.
-    + apply relax_ctx_bound with (t1 := t). eauto. unfold update_t; eauto.
-    + specialize (HH3 p). remember (mem p) as access eqn:ACCESS.
-      destruct access; eauto. destruct e0.
-      apply relax_ctx_bound with (t1 := t). apply HH3.
-      pose proof (p_bound_or_not p t) as CASES.
-      destruct CASES as [? | contra]; eauto. apply HH2 in contra.
-      rewrite contra in ACCESS. inversion ACCESS. unfold update_t. eauto.
-  - specialize (H BOUND).
-    destruct st. destruct st_m1. destruct st_m2.
-    simpl in BOUND. destruct BOUND as [B1 [B2 B3]].
-    simpl in H. destruct H as [HH1 [HH2 HH3]].
-    apply time_increase_m in EVALm1 as time_inc1.
-    apply time_increase_m in EVALm2 as time_inc2.
-    apply H0. simpl. repeat split; eauto.
+    simpl in IHEVAL1. destruct IHEVAL1 as [HH1 [HH2 HH3]].
+    apply time_increase_e in EVAL1 as time_inc1.
+    apply time_increase_e in EVAL2 as time_inc2.
+    apply IHEVAL2. simpl. repeat split; eauto.
     rewrite plugin_ctx_bound. split.
     apply relax_ctx_bound with (t1 := t); eauto.
     simpl; split; eauto.
@@ -506,18 +382,11 @@ Proof.
   - assert (α tx = α' tx). red in H. apply H. nia. rewrite H0. eauto.
 Qed.
 
-Lemma abs_eq_p_refl :
-  forall p,
-    Abstract.eq_p p p = true.
-Proof.
-  intros. apply Abstract.eq_p_eq. eauto.
-Qed.
-
 (* Set Printing Implicit. *)
 
 Lemma sound_eval :
-  forall C st e e' st'
-         (EVAL : EevalR C st e e' st')
+  forall C st e v' st'
+         (EVAL : EvalR C st e v' st')
          (BOUND : time_bound C st)
          abs_C abs_st α
          (SOUND : sound α C st abs_C abs_st),
@@ -525,58 +394,49 @@ Lemma sound_eval :
       match st with
       | ST _ t =>
         eq_bound_α t α α' /\
-        match e' with
-        | Val _ _ C' =>
-          sound α' C' st' abs_C' abs_st'
+        match v' with
+        | EVal (Closure x' e' C') =>
+          sound α' C' st' abs_C' abs_st' /\
+          Abstract.EvalR 
+            abs_C abs_st e 
+            (Abstract.EVal (Abstract.Closure x' e' (trans_ctx α' C')))
+            abs_st'
+        | MVal C' =>
+          sound α' C' st' abs_C' abs_st' /\
+          Abstract.EvalR 
+            abs_C abs_st e 
+            (Abstract.MVal (trans_ctx α' C'))
+            abs_st' 
         end
       end.
 Proof.
-  apply (EevalR_ind_mut 
-    (fun C st e e' st'
-         (EVAL : EevalR C st e e' st') =>
-    forall
-         (BOUND : time_bound C st)
-         abs_C abs_st α
-         (SOUND : sound α C st abs_C abs_st),
-    exists abs_C' abs_st' α',
-      match st with
-      | ST _ t =>
-        eq_bound_α t α α' /\
-        match e' with
-        | Val _ _ C' =>
-          sound α' C' st' abs_C' abs_st'
-        end
-      end)
-    (fun C st m C' st'
-         (EVAL : MevalR C st m C' st') =>
-    forall
-         (BOUND : time_bound C st)
-         abs_C abs_st α
-         (SOUND : sound α C st abs_C abs_st),
-    exists abs_C' abs_st' α',
-      match st with
-      | ST _ t =>
-        eq_bound_α t α α' /\
-        sound α' C' st' abs_C' abs_st'
-      end)); intros; subst.
+  intros. revert abs_C abs_st α SOUND. induction EVAL; intros; subst.
   - unfold sound in SOUND. destruct abs_st as [abs_mem abs_t].
     destruct SOUND as [? [? ?]].
     specialize (H1 (addr_x C x)) as HINT. rewrite <- ACCESS in HINT.
     destruct v as [v pf C'].
     exists (trans_ctx α C'). exists (Abstract.ST abs_mem abs_t). exists α.
-    split; red; intros; eauto.
-  - exists abs_C. exists abs_st. exists α. repeat split; eauto using Abstract.EevalR.
-    destruct st; simpl; split; red; intros; eauto.
-  - pose proof (time_bound_e C st e1 (Val (e_lam x e) (v_fn x e) C_lam) st_lam FN) as BOUND'.
-    pose proof (time_bound_e C st_lam e2 arg (ST mem t) ARG) as BOUND''.
+    repeat split; try red; intros; eauto. apply H1. eauto.
+    eapply Abstract.Eval_var_e; eauto.
+    rewrite <- H0. rewrite trans_ctx_addr.
+    destruct (addr_x C x). specialize (ADDR eq_refl). inversion ADDR.
+    simpl; unfold not; intros contra; inversion contra.
+    rewrite <- H0. rewrite trans_ctx_addr.
+    apply HINT. simpl in BOUND. destruct BOUND. apply time_bound_addr. eauto.
+  - exists abs_C. exists abs_st. exists α. repeat split; eauto using Abstract.EvalR.
+    destruct st; simpl; repeat split; try red; intros; eauto.
+    destruct abs_st. simpl in SOUND. destruct SOUND as [? [? ?]].
+    rewrite H0. eauto using Abstract.EvalR.
+  - pose proof (time_bound_e C st e1 (EVal (Closure x e C_lam)) st_lam EVAL1) as BOUND'.
+    pose proof (time_bound_e C st_lam e2 (EVal arg) (ST mem t) EVAL2) as BOUND''.
     pose proof (time_bound_e (C_lam [|dy_c_lam x t ([||])|])
-                             (ST (t :: dy_level C_lam !-> arg; mem) (update_t t))
-                             e v st_v BODY) as BOUND'''.
+                             (ST (t :: dy_level C_lam !-> arg; mem) (update_t C (ST mem t) x arg))
+                             e (EVal v) st_v EVAL3) as BOUND'''.
     specialize (BOUND' BOUND). simpl in BOUND'.
     destruct st. destruct st_lam. destruct st_v.
-    apply time_increase_e in ARG as time_inc1.
-    apply time_increase_e in FN as time_inc2.
-    apply time_increase_e in BODY as time_inc3.
+    apply time_increase_e in EVAL1 as time_inc1.
+    apply time_increase_e in EVAL2 as time_inc2.
+    apply time_increase_e in EVAL3 as time_inc3.
     assert (time_bound C (ST mem1 t1)) as B1. 
     { simpl. simpl in BOUND. destruct BOUND as [? [? ?]].
              simpl in BOUND'. destruct BOUND' as [? [? ?]].
@@ -585,10 +445,11 @@ Proof.
     specialize (BOUND'' B1).
     destruct arg. destruct v.
     assert (time_bound (C_lam [|dy_c_lam x t ([||])|])
-             (ST (t :: dy_level C_lam !-> Val v0 pf C0; mem) (update_t t))) as B2.
-    { simpl. simpl in BOUND. destruct BOUND as [? [? ?]].
-             simpl in BOUND'. destruct BOUND' as [? [? ?]].
-             simpl in BOUND''. destruct BOUND'' as [? [? ?]].
+             (ST (t :: dy_level C_lam !-> Closure x0 e0 C0; mem)
+                (update_t C (ST mem t) x (Closure x0 e0 C0)))) as B2.
+    { simpl. simpl in BOUND. destruct BOUND as [BB1 [BB2 BB3]].
+             simpl in BOUND'. destruct BOUND' as [BB1' [BB2' BB3']].
+             simpl in BOUND''. destruct BOUND'' as [BB1'' [BB2'' BB3'']].
       unfold update_t in *.
       split. rewrite plugin_ctx_bound. split.
       eapply relax_ctx_bound. eauto. eauto. simpl. split; eauto. split.
@@ -599,106 +460,323 @@ Proof.
       assert (t < S t /\ p_bound (dy_level C_lam) (S t)) as contra.
       split; eauto. apply time_bound_level. apply relax_ctx_bound with (t1 := t1). eauto. eauto.
       apply NBOUND in contra. inversion contra.
-      apply H9. unfold not. intros contra.
+      apply BB2''. unfold not. intros contra.
       assert (p_bound p (S t)). apply relax_p_bound with (t1 := t); eauto.
-      apply NBOUND in H11. inversion H11.
+      apply NBOUND in H. inversion H.
       (* bound, then access is bound *)
       intros. unfold update_m. remember (eq_p p (t :: dy_level C_lam)) as b.
       destruct b. symmetry in Heqb. rewrite eq_p_eq in Heqb.
       rewrite Heqb in BOUND. simpl in BOUND. destruct BOUND.
       apply relax_ctx_bound with (t1 := t); eauto.
-      pose proof (p_bound_or_not p t). 
-      remember (mem p) as access eqn:ACCESS. 
-      destruct H11; destruct access; try destruct e0; eauto;
-      try specialize (H10 p H11); try specialize (H9 p H11);
-      try rewrite <- ACCESS in H10; try rewrite <- ACCESS in H9; 
-      apply relax_ctx_bound with (t1 := t); eauto. inversion H9. }
+      pose proof (p_bound_or_not p t) as CASES.
+      remember (mem p) as access eqn:ACCESS.
+      destruct CASES; destruct access; try destruct e4; eauto;
+      try specialize (BB2'' p H); try specialize (BB3'' p H);
+      try rewrite <- ACCESS in BB2''; try rewrite <- ACCESS in BB3'';
+      try apply relax_ctx_bound with (t1 := t); eauto. inversion BB2''. }
     specialize (BOUND''' B2).
-    specialize (H BOUND). specialize (H0 B1). specialize (H1 B2). 
-    specialize (H abs_C abs_st α SOUND). 
-    destruct H as [abs_C' [abs_st' [α' [EQ' SOUND']]]].
+    specialize (IHEVAL1 BOUND). specialize (IHEVAL2 B1). specialize (IHEVAL3 B2). 
+    specialize (IHEVAL1 abs_C abs_st α SOUND).
+    destruct IHEVAL1 as [abs_C' [abs_st' [α' [EQ' SOUND']]]].
     assert (sound α' C (ST mem1 t1) abs_C abs_st').
-    { destruct abs_st'. simpl. simpl in SOUND'. destruct SOUND' as [? [? ?]].
+    { destruct abs_st'. simpl. simpl in SOUND'. destruct SOUND' as [[? [? ?]] ?].
       repeat split; eauto. destruct abs_st. simpl in SOUND. destruct SOUND as [? [? ?]].
-      rewrite <- H5. symmetry. eapply bound_trans_ctx_eq. simpl in BOUND. destruct BOUND.
+      rewrite <- H4. symmetry. eapply bound_trans_ctx_eq. simpl in BOUND. destruct BOUND.
       eauto. eauto. }
-    specialize (H0 abs_C abs_st' α' H). clear H.
-    destruct H0 as [abs_C'' [abs_st'' [α'' [EQ'' SOUND'']]]]. destruct abs_st'' as [mem'' t''].
+    specialize (IHEVAL2 abs_C abs_st' α' H). clear H.
+    destruct IHEVAL2 as [abs_C'' [abs_st'' [α'' [EQ'' SOUND'']]]]. destruct abs_st'' as [mem'' t''].
     remember (fun (t' : nat) => if t' =? S t 
-                        then Abstract.update_t (α'' t) else α'' t') as α'''.
+                        then Abstract.update_t abs_C (Abstract.ST mem'' t'') 
+                                                x (Abstract.Closure x0 e0 abs_C'') 
+                        else α'' t') as α'''.
     assert (sound α''' (C_lam [|dy_c_lam x t ([||])|])
-            (ST (t :: dy_level C_lam !-> Val v0 pf C0; mem) (update_t t))
+            (ST (t :: dy_level C_lam !-> Closure x0 e0 C0; mem) 
+                (update_t C (ST mem t) x (Closure x0 e0 C0)))
             (abs_C'[#| Abstract.dy_c_lam x (α'' t) ([#||#]) |#])
-            (Abstract.ST ((α'' t) :: Abstract.dy_level abs_C' !#-> Abstract.Val v0 pf abs_C''; mem'') (Abstract.update_t (α'' t)))).
+            (Abstract.ST ((α'' t) :: Abstract.dy_level abs_C' !#-> Abstract.Closure x0 e0 abs_C''; mem'') 
+                         (Abstract.update_t abs_C (Abstract.ST mem'' t'') x (Abstract.Closure x0 e0 abs_C'')))).
     { simpl. unfold update_t in *. repeat split.
       - rewrite Heqα'''. simpl. assert (t =? t = true). rewrite Nat.eqb_eq. eauto. rewrite H. eauto.
       - rewrite Heqα'''. simpl. rewrite plugin_trans_ctx; simpl.
         assert (t =? S t = false). rewrite Nat.eqb_neq. eauto. rewrite H.
         assert (trans_ctx α''' C_lam = abs_C'). rewrite Heqα'''.
-        destruct abs_st'. simpl in SOUND'. destruct SOUND' as [? [? ?]]. rewrite <- H2.
+        destruct abs_st'. simpl in SOUND'. destruct SOUND' as [[? [? ?]] ?]. rewrite <- H1.
         apply bound_trans_ctx_eq with (t := t1). simpl in BOUND'. destruct BOUND'. eauto.
         red. intros. assert (t' <> S t). nia. rewrite <- Nat.eqb_neq in H4. rewrite H4.
-        symmetry. apply EQ''. eauto. rewrite <- Heqα'''. rewrite H0. eauto.
-      - intros. simpl in SOUND''. destruct SOUND'' as [? [? ?]].
-        destruct abs_st'. simpl in SOUND'. destruct SOUND' as [? [? ?]].
+        symmetry. apply EQ''. eauto. 
+        rewrite Heqα''' in H0. simpl in H0. rewrite H0. eauto.
+      - intros. simpl in SOUND''. destruct SOUND'' as [[? [? ?]] ?].
+        destruct abs_st'. simpl in SOUND'. destruct SOUND' as [[? [? ?]] ?].
         unfold update_m. unfold Abstract.update_m.
         remember (eq_p p (t :: dy_level C_lam)) as b.
         destruct b. symmetry in Heqb. rewrite eq_p_eq in Heqb.
         assert (map α''' p =  α'' t :: Abstract.dy_level abs_C').
         rewrite Heqα'''. rewrite Heqb. simpl. assert (RR : t =? S t = false). 
         apply Nat.eqb_neq. eauto. rewrite RR. clear RR. rewrite <- H4.
-        assert (Abstract.dy_level (trans_ctx α' C_lam) = map (fun t' : nat =>
-                      if t' =? S t then Abstract.update_t (α'' t) else α'' t')
-                      (dy_level C_lam)) as RR.
+        assert (Abstract.dy_level (trans_ctx α' C_lam) = map α''' (dy_level C_lam)) as RR.
         apply level_trans_ctx_eq with (t := t1). red. intros.
-        assert (t' =? S t = false). rewrite Nat.eqb_neq. nia. rewrite H6. apply EQ''. eauto.
+        assert (t' =? S t = false). rewrite Nat.eqb_neq. nia.
+        rewrite Heqα'''. rewrite H7. apply EQ''. eauto.
         simpl in BOUND'. destruct BOUND'. eauto.
-        rewrite RR. eauto. rewrite <- H6.
+        rewrite RR. rewrite Heqα'''. simpl. eauto.
         (* A bug? in Coq : have to write explicitly the implicit parameters *)
         assert (Abstract.eq_p (@map time Abstract.time α''' p) (@map nat bool α''' p) = true).
-        rewrite Abstract.eq_p_eq. eauto. rewrite H7. simpl. left.
+        rewrite Abstract.eq_p_eq. eauto. rewrite <- H7. rewrite H8. simpl. left.
         assert (abs_C'' = trans_ctx α''' C0).
         rewrite <- H0. eapply bound_trans_ctx_eq. simpl in BOUND''. destruct BOUND''. eauto.
         rewrite Heqα'''. red. intros. assert (t' =? S t = false). rewrite Nat.eqb_neq. nia.
-        rewrite H8. eauto. rewrite H8. eauto.
+        rewrite H9. eauto. rewrite H9. eauto.
         pose proof (p_bound_or_not p t) as CASES.
         simpl in BOUND''. destruct BOUND'' as [B1'' [B2'' B3'']].
         destruct CASES as [L | R]; 
         try (specialize (B2'' p R); rewrite B2''; eauto; fail).
         remember (mem p) as access eqn: ACCESS.
-        destruct access; eauto; destruct e0; simpl.
-        specialize (H2 p L). rewrite <- ACCESS in H2.
+        destruct access; eauto; destruct e4; simpl.
+        specialize (H1 p L) as HINT. rewrite <- ACCESS in HINT.
         assert (@map time Abstract.time α''' p = map α'' p) as RR. 
-        { clear H2. clear BOUND0. clear Heqb. clear ACCESS.
+        { clear HINT. clear BOUND0. clear Heqb. clear ACCESS.
           induction p; simpl; eauto. simpl in L; destruct L.
           rewrite IHp; eauto. rewrite Heqα'''. 
           assert (a =? S t = false). rewrite Nat.eqb_neq. nia.
-          rewrite H7. eauto. } rewrite RR; clear RR.
+          rewrite H9. eauto. } rewrite RR; clear RR.
         assert (trans_ctx α''' C2 = trans_ctx α'' C2) as RR.
         { apply bound_trans_ctx_eq with (t := t).
           specialize (B3'' p L). rewrite <- ACCESS in B3''. eauto.
           rewrite Heqα'''. red. intros. assert (t' =? S t = false).
-          rewrite Nat.eqb_neq. nia. rewrite H6. eauto. } rewrite RR; clear RR.
+          rewrite Nat.eqb_neq. nia. rewrite H7. eauto. } rewrite RR; clear RR.
         remember (α'' t :: Abstract.dy_level abs_C') as p'.
         remember (Abstract.eq_p (map α'' p) p') as b.
         destruct b. 
         simpl. right. symmetry in Heqb0. rewrite Abstract.eq_p_eq in Heqb0.
-        rewrite <- Heqb0. apply H2. apply H2.
+        rewrite <- Heqb0. apply HINT. apply HINT.
     }
     assert (eq_bound_α t α'' α''') as EQ'''.
     { red. intros. rewrite Heqα'''. assert (t' =? S t = false). rewrite Nat.eqb_neq. nia.
       rewrite H0. eauto. }
-    specialize (H1 (abs_C' [#|Abstract.dy_c_lam x (α'' t) ([#||#])|#])
+    specialize (IHEVAL3 (abs_C' [#|Abstract.dy_c_lam x (α'' t) ([#||#])|#])
                 (Abstract.ST
                   (α'' t :: Abstract.dy_level abs_C'
-                      !#-> Abstract.Val v0 pf abs_C''; mem'')
-                  (Abstract.update_t (α'' t))) α''' H).
-    destruct H1 as [abs_C''' [abs_st''' [α'''' [EQ'''' SOUND''']]]].
-    exists abs_C'''. exists abs_st'''. exists α''''. split; eauto.
+                      !#-> Abstract.Closure x0 e0 abs_C''; mem'')
+                  (Abstract.update_t abs_C (Abstract.ST mem'' t'') x
+                  (Abstract.Closure x0 e0 abs_C''))) α''' H).
+    destruct IHEVAL3 as [abs_C''' [abs_st''' [α'''' [EQ'''' SOUND''']]]].
+    destruct SOUND' as [SOUND' EVAL'].
+    destruct SOUND'' as [SOUND'' EVAL''].
+    destruct SOUND''' as [SOUND''' EVAL'''].
+    exists abs_C'''. exists abs_st'''. exists α''''. repeat split; eauto.
     red. intros. 
     assert (α t' = α' t') as RR. apply EQ'. eauto. rewrite RR; clear RR.
     assert (α' t' = α'' t') as RR. apply EQ''. nia. rewrite RR; clear RR.
     assert (α'' t' = α''' t') as RR. apply EQ'''. nia. rewrite RR; clear RR.
     apply EQ''''. unfold update_t. nia.
-  - 
-  
+    eapply Abstract.Eval_app. exact EVAL'. exact EVAL''.
+    destruct abs_st'. simpl in SOUND'. destruct SOUND' as [? [RR ?]].
+    rewrite RR. simpl in SOUND''. destruct SOUND'' as [? [RR' ?]].
+    rewrite RR'. rewrite <- H2. rewrite <- H2 in EVAL'''. exact EVAL'''.
+  - pose proof (time_bound_e C st m (MVal C_m) st_m EVAL1) as BOUND'.
+    pose proof (time_bound_e C_m st_m e (EVal v) st_v EVAL2) as BOUND''.
+    specialize (BOUND' BOUND). simpl in BOUND'. 
+    specialize (BOUND'' BOUND'). simpl in BOUND''. destruct v.
+    destruct st. destruct st_m. destruct st_v.
+    apply time_increase_e in EVAL1 as time_inc1.
+    apply time_increase_e in EVAL2 as time_inc2.
+    specialize (IHEVAL1 BOUND abs_C abs_st α SOUND).
+    destruct IHEVAL1 as [abs_C' [abs_st' [α' [EQ' SOUND']]]].
+    destruct SOUND' as [SOUND' EVAL']. 
+    specialize (IHEVAL2 BOUND' abs_C' abs_st' α' SOUND').
+    destruct IHEVAL2 as [abs_C'' [abs_st'' [α'' [EQ'' SOUND'']]]].
+    destruct SOUND'' as [SOUND'' EVAL''].
+    exists abs_C''. exists abs_st''. exists α''. repeat split; eauto.
+    unfold eq_bound_α in *. intros.
+    assert (α'' t' = α' t'). symmetry. apply EQ''. nia.
+    rewrite H. apply EQ'. eauto.
+    eapply Abstract.Eval_link. eauto.
+    destruct abs_st'. simpl in SOUND'. destruct SOUND' as [? [RR ?]].
+    rewrite RR. eauto.
+  - exists abs_C. exists abs_st. exists α. destruct st.
+    repeat split; eauto. unfold eq_bound_α; intros; eauto.
+    destruct abs_st. simpl in SOUND. destruct SOUND as [? [RR ?]].
+    rewrite RR. eauto using Abstract.EvalR.
+  - exists (trans_ctx α C_M). exists abs_st. exists α. destruct st.
+    destruct abs_st. destruct SOUND as [? [RR ?]].
+    repeat split; eauto. rewrite <- RR.
+    eapply Abstract.Eval_var_m. erewrite trans_ctx_ctx_M; eauto.
+  - pose proof (time_bound_e C st e (EVal v) (ST mem t) EVAL1) as BOUND'.
+    pose proof (time_bound_e (C [|dy_c_lete x t ([||])|]) 
+                             (ST (t :: dy_level C !-> v; mem)
+                                 (update_t C (ST mem t) x v)) m
+                             (MVal C_m) st_m EVAL2) as BOUND''.
+    specialize (BOUND' BOUND). simpl in BOUND'.
+    destruct st. destruct st_m. destruct v.
+    apply time_increase_e in EVAL1 as time_inc1.
+    apply time_increase_e in EVAL2 as time_inc2.
+    assert (time_bound (C [|dy_c_lete x t ([||])|])
+            (ST (t :: dy_level C !-> (Closure x0 e0 C0); mem)
+               (update_t C (ST mem t) x (Closure x0 e0 C0)))) as B1.
+    { simpl. simpl in BOUND. destruct BOUND as [BB1 [BB2 BB3]].
+             simpl in BOUND'. destruct BOUND' as [BB1' [BB2' BB3']].
+      unfold update_t in *.
+      split. rewrite plugin_ctx_bound. split.
+      eapply relax_ctx_bound. eauto. eauto. simpl. split; eauto. split.
+      (* not bound, then None *)
+      intros. unfold update_m. remember (eq_p p (t :: dy_level C)) as b.
+      destruct b. symmetry in Heqb. rewrite eq_p_eq in Heqb.
+      rewrite Heqb in NBOUND. simpl in NBOUND.
+      assert (t < S t /\ p_bound (dy_level C) (S t)) as contra.
+      split; eauto. apply time_bound_level. apply relax_ctx_bound with (t1 := t0). eauto. eauto.
+      apply NBOUND in contra. inversion contra.
+      apply BB2'. unfold not. intros contra.
+      assert (p_bound p (S t)). apply relax_p_bound with (t1 := t); eauto.
+      apply NBOUND in H. inversion H.
+      (* bound, then access is bound *)
+      intros. unfold update_m. remember (eq_p p (t :: dy_level C)) as b.
+      destruct b. symmetry in Heqb. rewrite eq_p_eq in Heqb.
+      rewrite Heqb in BOUND. simpl in BOUND. destruct BOUND.
+      apply relax_ctx_bound with (t1 := t); eauto.
+      pose proof (p_bound_or_not p t) as CASES.
+      remember (mem p) as access eqn:ACCESS.
+      destruct CASES; destruct access; try destruct e1; eauto;
+      try specialize (BB2' p H); try specialize (BB3' p H);
+      try rewrite <- ACCESS in BB2'; try rewrite <- ACCESS in BB3';
+      try apply relax_ctx_bound with (t1 := t); eauto. inversion BB2'. }
+    specialize (BOUND'' B1).
+    specialize (IHEVAL1 BOUND). specialize (IHEVAL2 B1).
+    specialize (IHEVAL1 abs_C abs_st α SOUND).
+    destruct IHEVAL1 as [abs_C' [abs_st' [α' [EQ' SOUND']]]].
+    remember (fun (t' : nat) => if t' =? S t 
+                        then Abstract.update_t abs_C abs_st'
+                                                x (Abstract.Closure x0 e0 abs_C') 
+                        else α' t') as α''.
+    destruct abs_st as [mem' t']. destruct abs_st' as [mem'' t''].
+    assert (sound α'' (C [|dy_c_lete x t ([||])|])
+            (ST (t :: dy_level C !-> Closure x0 e0 C0; mem) 
+                (update_t C (ST mem t) x (Closure x0 e0 C0)))
+            (abs_C [#| Abstract.dy_c_lete x (α' t) ([#||#]) |#])
+            (Abstract.ST ((α' t) :: Abstract.dy_level abs_C !#-> Abstract.Closure x0 e0 abs_C'; mem'') 
+                         (Abstract.update_t abs_C (Abstract.ST mem'' t'') x (Abstract.Closure x0 e0 abs_C')))).
+    { simpl. unfold update_t in *. repeat split.
+      - rewrite Heqα''. simpl. assert (t =? t = true). rewrite Nat.eqb_eq. eauto. rewrite H. eauto.
+      - rewrite Heqα''. simpl. rewrite plugin_trans_ctx; simpl.
+        assert (t =? S t = false). rewrite Nat.eqb_neq. eauto. rewrite H.
+        assert (trans_ctx α'' C = abs_C). 
+        simpl in SOUND. destruct SOUND as [? [RR ?]]. rewrite <- RR.
+        apply bound_trans_ctx_eq with (t := t0). destruct BOUND. eauto.
+        red. intros. rewrite Heqα''. assert (t'0 <> S t) as RR'. nia. rewrite <- Nat.eqb_neq in RR'. rewrite RR'.
+        symmetry. apply EQ'. eauto. 
+        rewrite Heqα'' in H0. simpl in H0. rewrite H0. eauto.
+      - intros. simpl in SOUND. destruct SOUND as [? [? ?]].
+                simpl in SOUND'. destruct SOUND' as [[? [? ?]] ?].
+        unfold update_m. unfold Abstract.update_m.
+        remember (eq_p p (t :: dy_level C)) as b.
+        destruct b. symmetry in Heqb. rewrite eq_p_eq in Heqb.
+        assert (map α'' p =  α' t :: Abstract.dy_level abs_C).
+        rewrite Heqα''. rewrite Heqb. simpl. assert (RR : t =? S t = false). 
+        apply Nat.eqb_neq. eauto. rewrite RR. clear RR. rewrite <- H0.
+        assert (Abstract.dy_level (trans_ctx α C) = map α'' (dy_level C)) as RR.
+        apply level_trans_ctx_eq with (t := t0). red. intros.
+        rewrite Heqα''. assert (t'0 =? S t = false). rewrite Nat.eqb_neq. nia.
+        rewrite H6. apply EQ'. eauto.
+        simpl in BOUND. destruct BOUND. eauto.
+        rewrite RR. rewrite Heqα''. simpl. eauto.
+        (* A bug? in Coq : have to write explicitly the implicit parameters *)
+        assert (Abstract.eq_p (@map time Abstract.time α'' p) (@map nat bool α'' p) = true).
+        rewrite Abstract.eq_p_eq. eauto. rewrite <- H6. rewrite H7. simpl. left.
+        assert (abs_C' = trans_ctx α'' C0).
+        rewrite <- H3. eapply bound_trans_ctx_eq. simpl in BOUND'. destruct BOUND'. eauto.
+        rewrite Heqα''. red. intros. assert (t'0 =? S t = false). rewrite Nat.eqb_neq. nia.
+        rewrite H8. eauto. rewrite H8. eauto.
+        pose proof (p_bound_or_not p t) as CASES.
+        destruct BOUND' as [B1' [B2' B3']].
+        destruct CASES as [L | R]; 
+        try (specialize (B2' p R); rewrite B2'; eauto; fail).
+        remember (mem p) as access eqn: ACCESS.
+        destruct access; eauto; destruct e1; simpl.
+        specialize (H4 p L) as HINT. rewrite <- ACCESS in HINT.
+        assert (@map time Abstract.time α'' p = map α' p) as RR.
+        { clear HINT. clear BOUND0. clear Heqb. clear ACCESS.
+          induction p; simpl; eauto. simpl in L; destruct L.
+          rewrite IHp; eauto. rewrite Heqα''. 
+          assert (a =? S t = false). rewrite Nat.eqb_neq. nia.
+          rewrite H8. eauto. } rewrite RR; clear RR.
+        assert (trans_ctx α'' C1 = trans_ctx α' C1) as RR.
+        { apply bound_trans_ctx_eq with (t := t).
+          specialize (B3' p L). rewrite <- ACCESS in B3'. eauto.
+          rewrite Heqα''. red. intros. assert (t'0 =? S t = false).
+          rewrite Nat.eqb_neq. nia. rewrite H6. eauto. } rewrite RR; clear RR.
+        remember (α' t :: Abstract.dy_level abs_C) as p'.
+        remember (Abstract.eq_p (map α' p) p') as b.
+        destruct b. 
+        simpl. right. symmetry in Heqb0. rewrite Abstract.eq_p_eq in Heqb0.
+        rewrite <- Heqb0. apply HINT. apply HINT.
+    }
+    assert (eq_bound_α t α' α'') as EQ''.
+    { red. intros. rewrite Heqα''. assert (t'0 =? S t = false). rewrite Nat.eqb_neq. nia.
+      rewrite H0. eauto. }
+    specialize (IHEVAL2 (abs_C [#|Abstract.dy_c_lete x (α' t) ([#||#])|#])
+                (Abstract.ST
+                  (α' t :: Abstract.dy_level abs_C
+                      !#-> Abstract.Closure x0 e0 abs_C'; mem'')
+                  (Abstract.update_t abs_C (Abstract.ST mem'' t'') x
+                  (Abstract.Closure x0 e0 abs_C'))) α'' H).
+    destruct IHEVAL2 as [abs_C'' [abs_st'' [α''' [EQ''' SOUND''']]]].
+    destruct SOUND' as [SOUND' EVAL'].
+    destruct SOUND''' as [SOUND''' EVAL'''].
+    exists abs_C''. exists abs_st''. exists α'''. repeat split; eauto.
+    red. intros. 
+    assert (α t'0 = α' t'0) as RR. apply EQ'. eauto. rewrite RR; clear RR.
+    assert (α' t'0 = α'' t'0) as RR. apply EQ''. nia. rewrite RR; clear RR.
+    apply EQ'''. unfold update_t. nia.
+    eapply Abstract.Eval_lete; eauto.
+    destruct SOUND' as [? [RR ?]]. rewrite RR. 
+    destruct abs_st''. destruct SOUND''' as [? [RR' ?]]. rewrite RR' in *.
+    rewrite <- H2. rewrite <- H2 in EVAL'''.
+    rewrite <- H0 in *. exact EVAL'''.
+  - pose proof (time_bound_e C st m' (MVal C') st' EVAL1) as BOUND'.
+    pose proof (time_bound_e (C [|dy_c_letm M C' ([||])|]) st' m''
+                             (MVal C'') st'' EVAL2) as BOUND''.
+    specialize (BOUND' BOUND). simpl in BOUND'.
+    destruct st. destruct st'. destruct st''.
+    apply time_increase_e in EVAL1 as time_inc1.
+    apply time_increase_e in EVAL2 as time_inc2.
+    assert (time_bound (C [|dy_c_letm M C' ([||])|])
+            (ST mem0 t0)) as B1.
+    { simpl. simpl in BOUND. destruct BOUND as [BB1 [BB2 BB3]].
+             simpl in BOUND'. destruct BOUND' as [BB1' [BB2' BB3']].
+      unfold update_t in *.
+      split. rewrite plugin_ctx_bound. split.
+      eapply relax_ctx_bound. eauto. eauto. simpl. split; eauto. split; eauto. }
+    specialize (BOUND'' B1).
+    specialize (IHEVAL1 BOUND). specialize (IHEVAL2 B1).
+    specialize (IHEVAL1 abs_C abs_st α SOUND).
+    destruct IHEVAL1 as [abs_C' [abs_st' [α' [EQ' SOUND']]]].
+    assert (sound α' (C [|dy_c_letm M C' ([||])|]) (ST mem0 t0)
+            (abs_C [#| Abstract.dy_c_letm M abs_C' ([#||#]) |#]) abs_st').
+    { unfold sound in *. destruct abs_st'. destruct abs_st.
+      destruct SOUND' as [[? [? ?]] ?].
+      destruct SOUND as [? [? ?]].
+      repeat split; simpl; eauto.
+      rewrite plugin_trans_ctx. simpl.
+      assert (trans_ctx α' C = abs_C).
+      rewrite <- H4. apply bound_trans_ctx_eq with (t := t).
+      simpl in BOUND. destruct BOUND; eauto. 
+      red; intros. red in EQ'. symmetry; apply EQ'; eauto.
+      rewrite H6.
+      assert (trans_ctx α' C' = abs_C').
+      rewrite <- H0. eauto. rewrite H7. eauto.
+    }
+    assert (eq_bound_α t α' α') as EQ''.
+    { red. intros; eauto. }
+    specialize (IHEVAL2 (abs_C [#|Abstract.dy_c_letm M abs_C' ([#||#])|#])
+                        abs_st' α' H).
+    destruct IHEVAL2 as [abs_C'' [abs_st'' [α'' [EQ''' SOUND''']]]].
+    destruct SOUND' as [SOUND' EVAL'].
+    destruct SOUND''' as [SOUND''' EVAL'''].
+    exists abs_C''. exists abs_st''. exists α''. repeat split; eauto.
+    red. intros. 
+    assert (α t' = α' t') as RR. apply EQ'. eauto. rewrite RR; clear RR.
+    apply EQ'''. unfold update_t. nia.
+    eapply Abstract.Eval_letm; eauto.
+    destruct abs_st'. destruct SOUND' as [? [RR ?]].
+    destruct abs_st''. destruct SOUND''' as [? [RR' ?]].
+    rewrite RR in *. rewrite RR' in *. eauto.
+Qed.
