doc/coq/Linking.v
@@ -1,0 +1,12 @@
+From MODULAR Require Import Concrete.
+
+Fixpoint inject_ctx Cout Cin :=
+  match Cin with
+  | ([||]) => Cout
+  | dy_c_lam x t C' =>
+    inject_ctx (Cout [|dy_c_lam x t ([||])|]) C'
+  | dy_c_lete x t C' =>
+    inject_ctx (Cout [|dy_c_lete x t ([||])|]) C'
+  | dy_c_letm M CM C' => 
+    inject_ctx (Cout [|dy_c_letm M (inject_ctx Cout CM) ([||])|]) C'
+  end.
